core done, just have to tidy up

Ownership-Lemmata.dfy
@@ -38,3 +38,198 @@ lemma AllReadyMeansEachObject1(os : Owner)
  requires AllReady(os)
   ensures forall o <- os :: o in o.AMFO
 {}
+
+
+
+
+
+lemma {:isolate_assertions} SubAMFOsNonU(partO : OWNR, wholeO : OWNR)
+    //partO is the "key" we're copying, "wholeO" is the piivo, top of the object ot b cloned
+    requires partO > wholeO  //ownerws trictk inside OWNR- sees to work either way!
+     ensures sub(partO,wholeO) + wholeO == partO
+{}
+
+lemma FlattenEq4(l : Owner, r : Owner, fl : OWNR, fr : OWNR)
+   requires  l == r
+   requires fl == flatten(l)
+   requires fr == flatten(r)
+    ensures fl == fr
+{}
+
+lemma FlattenEq2(l : Owner, r : Owner)
+   requires  l == r
+    ensures flatten(l) == flatten(r)
+{}
+
+// lemma NEWFlatten0(a : Object)
+//   requires a.AMFX == flatten(a.owner)
+//   requires a.AMFO == a.AMFX + {a}
+//    ensures flatten(a.self) == a.AMFO
+// {}
+
+lemma Flatten0(a : Object)
+  requires a.Ready()
+   ensures flatten(a.self) == a.AMFO
+{}
+
+// lemma Flatten1(a : Object)         //REVERT
+//   ensures flatten({a})    == a.AMFO     //REVERT
+// {}     //REVERT
+
+lemma Flatten2(a : Owner, b : Owner)
+  ensures flatten(a) + flatten(b) == flatten(a+b)
+{}
+
+lemma FlattenIncludesArgument(o : Owner)
+   ensures o <= flatten(o)
+    {}
+
+lemma {:isolate_assertions} FlattenExtraReady(o : Object)
+     requires o.Ready()
+      ensures o.self  <= o.AMFO
+      ensures o.owner <= o.AMFX <= o.AMFO
+      ensures o.bound <= o.AMFB <= o.AMFX <= o.AMFO
+    {}
+
+lemma FlatMeFlatMyOwners(o : Object,  oo : Owner)
+  requires o.Ready()
+  requires AllReady(oo)
+  requires isFlat(oo)
+
+  requires o in oo
+   ensures o.AMFO <= oo
+{}
+
+predicate AllTheseOwnersAreFlatOK(os : set<Object>, context : set<Object> := os)
+{ && flatten(os) <= context }
+
+
+
+lemma AMFOsisAMFOs(o : Object)
+  requires o.Ready()
+  ensures forall oo <- o.AMFO | oo != o :: (o.AMFO > oo.AMFO)
+  ensures forall oo <- o.AMFO | oo != o :: strictlyInside(o, oo)
+  ensures forall oo <- o.AMFO           :: inside(o, oo)
+{}
+
+///=====================================================================================
+///
+/// spare stuff that as lurking in Ownership that seems pretty damn preipheral.
+///  dunno how much is needed vs how much is junk vs how much is
+///
+///=====================================================================================
+///=====================================================================================
+///=====================================================================================
+
+
+
+
+
+
+
+
+
+
+
+
+
+
+
+
+
+
+
+
+
+
+
+
+
+
+
+
+
+
+
+
+
+
+
+
+
+
+lemma DirectlyInside(part : Object, whole : Object)
+  requires part.Ready()
+  requires whole.Ready()
+  requires directlyInside(part, whole)
+   ensures inside(part,whole)
+   ensures strictlyInside(part,whole)
+{
+//  FlattenInsideFlat(whole,flatten(part.owner));
+}
+
+lemma OnlyInside(part : Object, whole : Object)
+  requires part.Ready()
+  requires whole.Ready()
+  requires onlyInside(part, whole)
+   ensures inside(part,whole)
+   ensures strictlyInside(part,whole)
+{
+  // FlattenInsideFlat(whole,flatten(part.owner));
+}
+
+
+
+
+lemma {:isolate_assertions } DreddOwner(whole : Object, part : Object)
+  //NOTE argumenets are backwards, order is f->t not  part / whole
+  //if whole (f) inside part(t) owner list then...whole (directly )owns part
+  requires whole.Ready()
+  requires part.Ready()
+  requires whole in part.owner
+   ensures whole in flatten(part.owner)
+   ensures flatten({whole}) <= flatten(part.owner) < flatten({part})
+   ensures flatten({part}) > flatten(part.owner) >= flatten({whole})
+   ensures part.AMFO > part.AMFX >= whole.AMFO
+   ensures ownerInsideOwner(flatten(part.owner), flatten({whole}))
+   ensures inside(part,whole)
+{
+}
+
+
+lemma FlattenInsideFlat(f : Object, fs : Owner)
+  // (f in fs && isFlat(fs)) ==> (flatten({f}) <= fs)
+  requires f.Ready()
+  requires AllReady(fs)
+   ensures ((f in fs && isFlat(fs)) ==> (flatten({f}) <= fs))
+  requires isFlat(fs)
+  requires f in fs
+   ensures flatten({f}) <= fs
+{}
+
+
+
+lemma ownerInsideSanity(part : Object, whole : Object)
+  requires part.Ready()
+  requires whole.Ready()
+   ensures inside(part, whole)        ==> ownerInside(part.owner, whole.owner)
+   ensures inside(part, whole)       <==> ownerInside(part.self , whole.self )
+   ensures (part.AMFB >= whole.AMFB) <==> ownerInside(part.bound, whole.bound)
+  {}
+
+
+
+
+lemma InsideObjectsInsideOwners0(part : Object, whole : Object)
+  //CULL requires part.Ready()
+  //CULL requires whole.Ready()
+   ensures inside(part,whole) == ownerInsideOwner(part.AMFO, whole.AMFO)
+{}
+
+lemma {:isolate_assertions} InsideObjectsInsideOwners1(f : Object, t : Object)
+  requires f.Ready()
+  requires t.Ready()
+  requires f.AMFB >  t.AMFX //REENLAND
+///  requires f.AMFO >= t.AMFX   ///WRONG assic O-as-D, f->t ==> f inside T.owner
+   ensures refOK(f,t)
+{}
