Klon-Lemmata.dfy
@@ -1,0 +1,715 @@
+include "Klon.dfy"
+
+
+///////// basic
+
+lemma MapThruKlonIsVMap(kk: set<Object>, m : Klon, vv : set<Object>)
+  requires kk <= m.m.Keys
+  requires mapThruKlon(kk, m) == vv
+   ensures mapThruVMap(kk, m.m) == vv
+   {}
+
+lemma {:isolate_assertions} HNSV(v : Object, m : Klon)
+  ensures v in m.hns({v})
+  {}
+
+
+
+
+/////// (con)versions?
+
+
+lemma {:isolate_assertions} OwnersFromCalid(m : Klon)
+  requires m.SuperCalidFragilistic()
+   ensures m.SuperCalidOwners()
+   ensures m.CalidOwners()
+{
+    assert m.preOwners();
+    assert m.preOwners2();
+    assert (m.m.Keys <= m.oHeap);
+    assert m.objectInKlown(m.o);
+    assert m.AllLinesCalid();
+    assert (forall k <- m.m.Keys :: m.OwnersLineKV(k, m.m[k]));
+}
+
+
+lemma {:isolate_assertions} {:timeLimit 40} CalidFromOwners(m : Klon)
+  requires m.CalidOwners()
+  requires m.HeapContextReady()
+  requires m.ValuesContextReady()
+   ensures m.SuperCalidFragilistic()
+{
+    assert (forall k <- m.m.Keys :: m.OwnersLineKV(k, m.m[k]));
+    assert m.preOwners();
+    assert m.preOwners2();
+    assert (m.m.Keys <= m.oHeap);
+    assert m.objectInKlown(m.o);
+    assert forall k <- m.m.Keys :: (k.AMFX <= m.m.Keys) && (k.AMFB <= m.m.Keys);
+
+//                assert forall k <- m.m.Keys :: (
+
+  forall k <- m.m.Keys ensures (m.CalidLineKV(k,m.m[k]))
+    //by
+            {
+                      //body of CalidLIneKV as of 25 Jan 2026
+                      var v := m.m[k];
+ assert               && (k in m.oHeap)
+                      && (not(inside(k,m.o)) ==> (v == k))
+                      && (   (inside(k,m.o)) ==> (v !in m.oHeap))
+                  //    && (   (inside(k,o)) ==> (v.AMFO  >= v.AMFB >= k.AMFB))  //Beady2() GREENLAND
+                      && (   (inside(k,m.o)) ==> (k.AMFB <= m.o.AMFB) )  // GREENLAND Beady2()  GREENLAND -
+                      && (k.AMFX <= m.m.Keys)
+                      && (k.AMFB <= m.m.Keys)
+                      && (m.ownersInKlown(k))  //belt and braces--- currently a requirement!
+                      && (checkOwnershipOfClone(k,v, m))
+                      && (checkBoundOfClone(k,v, m))
+                      && (mappingOwnersThruKlownKV(k,v, m))
+                   ;
+    assert m.AllLinesCalid();
+     }
+}
+
+lemma {:isolate_assertions} OwnersLineFromCalidLine(k : Object, v : Object, m : Klon)
+    requires m.apoCalidse()
+    requires k.Ready()// && k.Valid() // should context go in here too? probasbly?
+    requires m.ownersInKlown(k)
+    requires v.Ready()
+    requires v in m.hns({v})
+    requires m.CalidLineKV(k,v)
+     ensures m.OwnersLineKV(k,v)
+    {}
+
+//// mappings
+
+lemma MapThruKlonFrom(os: set<Object>, m : Klon, m' : Klon)
+  requires os <= m'.m.Keys
+  requires m.from(m')
+  ensures  mapThruKlon(os, m) == mapThruKlon(os, m')
+{}
+
+lemma MapThruKlonFUCKED(os: set<Object>, ot : set<Object>,  m : Klon)
+  requires os <= m.m.Keys
+  requires ot <= m.m.Keys
+  requires os == ot
+  ensures  mapThruKlon(os, m) == mapThruKlon(ot, m)
+{}
+
+lemma MapThruKlonLEQ(os: set<Object>, ot : set<Object>,  m : Klon)
+  requires os <= m.m.Keys
+  requires ot <= m.m.Keys
+  requires os <= ot
+  ensures  mapThruKlon(os, m) <= mapThruKlon(ot, m)
+{}
+
+
+lemma MapThruKlonGEQ(os: set<Object>, ot : set<Object>,  m : Klon)
+  requires os <= m.m.Keys
+  requires ot <= m.m.Keys
+  requires os >= ot
+  ensures  mapThruKlon(os, m) >= mapThruKlon(ot, m)
+{}
+
+
+lemma MapThruKlonID(os: set<Object>, m : Klon)
+  requires os <= m.m.Keys
+  requires forall x <- os :: m.m[x] == x
+  ensures  mapThruKlon(os, m) == os
+{}
+
+
+lemma MapThruKlonIsMapThruVMap(ks: set<Object>, m : Klon, vs : set<Object>)
+  requires ks <= m.m.Keys
+  requires mapThruKlon(ks, m)   == vs
+  ensures  mapThruVMap(ks, m.m) == vs
+{}
+
+
+
+lemma ThereAndKlonAgain1(os: set<Object>, m : Klon, r : set<Object>)
+  requires os <= m.m.Keys
+  requires r  == mapThruKlon(os,m)
+   ensures r  <= m.m.Values
+   ensures os == mapBackKlon(r,m)
+{
+  InversionLove(m.m, invert(m.m));
+  assert r  == mapThruKlon(os,m);
+  assert os == mapBackKlon(r,m);
+}
+
+lemma ThereAndKlonAgain2(os: set<Object>, m : Klon, r : set<Object>)
+  requires os <= m.m.Values
+  requires r == mapBackKlon(os,m)
+   ensures r  <= m.m.Keys
+   ensures os  == mapThruKlon(r,m)
+ {
+    InversionLove(m.m, invert(m.m));
+ }
+
+
+
+
+//SuperDuperMappers --- well on the way but could do with a bnit more qwork
+
+lemma {:isolate_assertions} SuperDuperExternalMapperKV(k : Object, v : Object, m : Klon)
+  //outside stuff is maping. (and equa;)
+    requires m.apoCalidse()
+    requires m.ownersReadyInKlown(k)
+    requires m.SuperCalidFragilistic()
+    requires v.owner == computeOwnerForClone(k.owner, m)
+    requires v.bound == computeOwnerForClone(k.bound, m)
+    requires outside(k, m.o)
+     ensures mappingOWNRsThruKlownKV(k.owner,v.owner,m)
+     ensures mappingOWNRsThruKlownKV(k.bound,v.bound,m)
+{}
+
+
+lemma {:isolate_assertions} SuperDuperPivotMapperKV(k : Object, v : Object, m : Klon)
+  //consistency lemma… or somesthing.
+    requires m.apoCalidse()
+    requires m.ownersReadyInKlown(k)
+    requires m.SuperCalidFragilistic()
+    requires v.owner == computeOwnerForClone(k.owner, m)
+    requires v.bound == computeOwnerForClone(k.bound, m)
+    requires k == m.o
+     ensures mappingOWNRsThruKlownKV(k.owner,v.owner,m)
+     ensures mappingOWNRsThruKlownKV(k.bound,v.bound,m)
+{}
+
+
+lemma {:isolate_assertions} SuperDuperKlonMapperKV(m : Klon)
+  //consistency lemma… or somesthing.kkkkk
+    requires m.apoCalidse()
+    requires m.ownersReadyInKlown(m.o)
+    requires m.SuperCalidFragilistic()
+// i  ensures mappingOWNRsThruKlownKV(m.o.owner,m.m[m.o].owner,m)
+//     ensures mappingOWNRsThruKlownKV(m.o.bound,m.m[m.o].bound,m)
+     ensures m.m[m.o].owner == m.clowner
+     ensures m.m[m.o].bound == m.clbound
+{}
+
+
+
+lemma {:isolate_assertions} SuperDuperOwnerMapperKV(k : Object, v : Object, m : Klon)
+  //consistency lemma… or somesthing.
+    requires m.apoCalidse()
+    requires m.ownersReadyInKlown(k)
+    requires m.SuperCalidFragilistic()
+    requires k.Ready()
+    requires v.Ready()
+    requires m.CalidLineKV(k,v)
+    requires m.OwnersLineKV(k,v)
+//  requires v.owner == computeOwnerForClone(k.owner, m)
+//  requires v.bound == computeOwnerForClone(k.bound, m)
+     ensures mappingOwnersThruKlownKV(k,v,m)
+     ensures (k == m.o) ==> (
+          && (v == m.m[m.o])
+          && (v.owner == m.clowner)
+          && (v.bound == m.clbound))
+     ensures (outside(k, m.o)) ==> (v == k)
+     ensures (strictlyInside(k, m.o)) ==> (
+          && mappingOWNRsThruKlownKV(k.owner,v.owner,m)
+          && mappingOWNRsThruKlownKV(k.bound,v.bound,m)
+          && v.owner == computeOwnerForClone(k.owner, m)
+          && v.bound == computeOwnerForClone(k.bound, m)
+         )
+{}
+
+
+lemma {:isolate_assertions}  MappingInsideOwnersThruKlown(k : Object, v : Object, m : Klon)
+   decreases k.AMFO
+    requires k.Ready()
+    requires v.Ready()
+    requires m.apoCalidse()
+    requires m.ownersReadyInKlown(k)
+    requires strictlyInside(k, m.o)
+    requires k in m.m.Keys
+    requires m.m[k] == v
+
+      ensures strictlyInside(v, m.m[m.o])
+
+      requires mappingOwnersThruKlownKV(k,v,m)
+      requires mappingOWNRsThruKlownKV(k.owner, v.owner, m)
+      ensures forall oo <- k.owner | strictlyInside(oo,m.o) :: m.m[oo] in v.owner
+      ensures inside(v, m.m[m.o])
+  {
+    assert v.owner == (set x <- (k.owner - m.o.AMFO) :: m.m[x]) + m.m[m.o].AMFO;
+  }
+
+
+
+
+
+
+
+lemma {:isolate_assertions} MappedBounds(k : Object, v : Object, m : Klon)
+    requires k.Ready()
+    requires v.Ready()
+    requires m.ownersInKlown(k)
+    requires m.SuperCalidFragilistic()
+
+    requires strictlyInside(k, m.o)
+     ensures k.AMFO > m.o.AMFO
+
+    // ensures (forall oo <- k.AMFX :: k.AMFB <= oo.AMFB)  //GREENLAND //Beady2()
+    ensures nuBoundsOK(k.owner, k.bound)
+
+    requires mappingOWNRsThruKlownKV(k.owner, v.owner, m)
+   //  ensures (forall oo <- v.AMFX :: v.AMFB <= oo.AMFB)  //GREENLAND //Beady2()
+       ensures nuBoundsOK(v.owner, v.bound)
+  {
+    k.ExtraReady();  //GREENLAND //Beady2()
+    v.ExtraReady();  //GREENLAND //Beady2()
+    assert nuBoundsOK(k.owner, k.bound);
+    assert nuBoundsOK(v.owner, v.bound);
+//    assert (forall oo <- k.AMFX :: k.AMFB <= oo.AMFB + k.owner);   //GREENLAND //Beady2()
+//    assert (forall oo <- v.AMFX :: v.AMFB <= oo.AMFB + v.owner);  //GREENLAND //Beady2()
+
+    assert  k.AMFX >= k.AMFB;
+    assert  (forall oo <- k.AMFX :: oo in m.m.Keys);
+    assert  m.HeapContextReady();
+    assert  m.ValuesContextReady();
+    assert  AllReady(m.hns());
+
+    var nuowner := computeOwnerForClone(k.owner,m);
+    assert nuowner <= m.hns();
+    assert  AllReady(nuowner);
+    assert  AllReady(flatten(nuowner));
+    var nubound := computeOwnerForClone(k.bound,m);
+    assert nubound <= m.hns();
+    assert  AllReady(nubound);
+    assert  AllReady(flatten(nubound));
+    var fvbound := flatten(nubound);
+    var fvowner := flatten(nuowner);
+
+    assert nuowner == global(sideways(local(k.owner, m),m),m);
+    assert nubound == global(sideways(local(k.bound, m),m),m);
+
+
+
+    //  assert fvowner >= fvbound;                                  //THULE  //TODO
+    //  assert (forall vo <- fvowner :: fvbound <= vo.AMFB);        //THULE  //TODO
+
+//    assert fvbound >= collectBounds(fvowner);  //TODO NUBIOUBNDS...
+  }
+
+
+lemma {:isolate_assertions}  MappingSameObjectIsOutsideThruKlown(k : Object, v : Object, m : Klon)
+//wrong turn on the rocky road to dublin…
+//answer - it works cos saying  m.m[k] == k == v
+// constraints the spec so there are no solutions - except outside?
+   decreases k.AMFO
+    requires k.Ready()
+    requires v.Ready()
+    requires m.SuperCalidFragilistic()
+    requires m.objectReadyInKlown(k)
+    requires m.m[k] == k == v
+
+    ensures outside(k, m.o)
+{
+   assert m.AllLinesCalid();
+   assert m.CalidLineKV(k,v);
+   assert mappingOwnersThruKlownKV(k, v, m);
+}
+
+lemma {:isolate_assertions}  MappingInsideBoundsThruKlown(k : Object, v : Object, m : Klon)
+//wrong turn on the rocky road to dublin…
+//answer - it works cos saying "outside" overconstraints the spec so there are no solutions
+//saying m.m[k] == v gives us outside
+   decreases k.AMFO
+    requires k.Ready()
+    requires v.Ready()
+    requires m.apoCalidse()
+    requires m.ownersReadyInKlown(k)
+    // requires strictlyInside(k, m.o)  //how the hell does it work without this?
+
+    //requires outside(k, m.o)
+
+    requires k in m.m.Keys
+    requires m.m[k] == v
+
+    ensures flatten(k.owner) >= flatten(k.bound)
+    ensures flatten(v.owner) >= flatten(v.bound)
+
+    ensures strictlyInside(v, m.m[m.o])
+
+    requires mappingOwnersThruKlownKV(k,v,m)
+    requires mappingOWNRsThruKlownKV(k.bound, v.bound, m)
+    requires mappingOWNRsThruKlownKV(k.owner, v.owner, m)
+
+    ensures forall oo <- k.owner | strictlyInside(oo,m.o) :: m.m[oo] in v.owner
+    ensures inside(v, m.m[m.o])
+  {
+    assert v.owner == (set x <- (k.owner - m.o.AMFO) :: m.m[x]) + m.m[m.o].AMFO;
+}
+
+
+
+
+
+
+//// less basic
+
+
+
+lemma {:isolate_assertions} OwnershipOfCloneGEQ(os: set<Object>, ot : set<Object>,  m : Klon)
+//
+///kj 7 June 2025 - not claer how this  works if we're comaring owners and bounds?
+  requires os <= m.m.Keys <= m.oHeap
+  requires ot <= m.m.Keys <= m.oHeap
+  requires os >= ot
+
+  requires m.apoCalidse()
+  requires m.SuperCalidFragilistic()
+
+  requires m.m.Values <= m.hns()
+  requires m.o.Ready()
+  requires m.objectInKlown(m.o)
+  requires m.HeapOwnersReady()
+  requires m.c_amfx <= m.oHeap  //flattened ownershio of the top of the clone... - 'tis OK cos its the very top
+   ensures computeOwnerForClone(os, m) >= computeOwnerForClone(ot, m)
+{}
+
+
+
+
+
+lemma {:isolate_assertions} OwnershipOfCloneGEQ2(os: set<Object>, ot : set<Object>, m : Klon, ro : set<Object>, rt : set<Object>)
+  requires os <= m.m.Keys <= m.oHeap
+  requires ot <= m.m.Keys <= m.oHeap
+  requires os >= ot
+
+  requires m.apoCalidse()
+  requires m.SuperCalidFragilistic()
+
+  requires m.m.Values <= m.hns()
+  requires m.o.Ready()
+  requires m.objectInKlown(m.o)
+  requires m.HeapOwnersReady()
+  requires m.c_amfx <= m.oHeap  //flattened ownershio of the top of the clone... - 'tis OK cos its the very top
+
+   requires ro == computeOwnerForClone(os, m)
+   requires rt == computeOwnerForClone(ot, m)
+
+   ensures computeOwnerForClone(os, m) >= computeOwnerForClone(ot, m)
+{}
+
+
+
+
+
+
+
+
+//timelimit 60 BUT IT WORDS - 2 Jan 2026
+//but it doesn't 5 Mar 2026
+lemma {:isolate_assertions}  {:timeLimit 60} BROKENCalidKVCalid(k : Object, v : Object, m0 : Klon, m1 : Klon)
+  //if m0.klonKLV(kv == m1,  and m0 is calid, can m1 pretty please be calid()?
+    requires m0.CKV_preconditions(k,v)
+    requires m0.apoCalidse()
+    requires k.Ready()// && k.Valid() // should context go in here too? probasbly?
+    requires m0.ownersInKlown(k)
+    requires v.Ready()
+    requires m0.Calid()
+    requires m0.CalidLineKV(k,v)
+    requires k !in m0.m.Keys
+    requires v !in m0.m.Values
+    requires v in  m0.hns({v})
+    requires m1.from(m0)
+    requires m1 == klonKV(m0,k,v)
+     ensures m1.m == vmapKV(m0.m,k,v)
+     ensures k in m1.m.Keys
+     ensures m1.m.Keys   == m0.m.Keys + {k}
+     ensures m1.m.Values == m0.m.Values + {v}
+     ensures m1.m[k] == v
+     ensures m1.objectInKlown(k)
+     ensures m1.Calid()
+    {
+      assert m0.AllLinesCalid();
+      assert m0.CalidLineKV(k,v);
+        assert m0.gettingThere();
+      assert && (k.Ready())
+               && (m0.ownersInKlown(k))
+               && (v.Ready())
+               && (v in m0.hns({v}));
+
+      assert (k.Ready());
+      assert (m1.ownersInKlown(k));
+      assert (v.Ready());
+      assert (v in m1.hns({v}));
+
+      assert k in m1.m.Keys;
+      assert m1.objectInKlown(k);
+
+      assert m1.m.Keys == m0.m.Keys + {k};
+
+      forall j <- m1.m.Keys ensures (
+                              && (j.Ready())
+                              && (m1.objectInKlown(j))
+                              && (m1.m[j].Ready())
+                              && (m1.m[j] in m1.hns())
+                              && (m1.CalidLineKV(j,m1.m[j]))
+                                   )
+        {
+         if (j == k)
+           { assert m0.CalidLineKV(j,v);
+             m0.CalidLineKVTo(j,v,m1);
+             assert m1.CalidLineKV(j,v);
+             assert m1.m[j] == v;
+             assert m1.CalidLineKV(j,m1.m[j]);
+           } else {
+             assert j in m0.m.Keys;
+             assert m0.m[j] == m1.m[j];
+             assert m0.AllLinesCalid();
+             assert m0.CalidLineKV(j,m0.m[j]);
+             m0.CalidLineKVTo(j,m1.m[j],m1);
+             assert m1.CalidLineKV(j,m1.m[j]);
+           }
+        }
+
+        assert m1.gettingThere();
+
+        assert m0.ValuesContextReady();
+        assert m1.m.Values == m0.m.Values + {v};
+        assert m1.hns() == m0.hns({v});
+          assert v.Context(m0.hns({v}));
+        assert v.Context(m1.hns());
+//      assert forall x <- m0.m.Values :: x.Context(m0.hns()) && x.Context(m1.hns());
+        forall  x <- m0.m.Values ensures (x.Context(m1.hns())) //by
+          {
+            assert x.Context(m0.hns());
+            x.WiderContext(m0.hns(), m1.hns());
+            assert x.Context(m1.hns());
+          }
+        assert forall x <- m1.m.Values ::
+           if (x in m0.m.Values)
+              then (x.Context(m1.hns()))
+              else ((x == v) && (x.Context(m1.hns())));
+        assert m1.ValuesContextReady();
+  }
+
+
+
+lemma {:isolate_assertions} {:timeLimit 0} BETTERCalidKVCalid(k : Object, v : Object, m0 : Klon, m1 : Klon)
+  //if m0.klonKLV(kv == m1,  and m0 is calid, can m1 pretty please be calid()?
+    requires m0.CKV_preconditions(k,v)
+//requires HighCalidFragilistic(m0)
+    requires m0.apoCalidse()
+    requires k.Ready()// && k.Valid() // should context go in here too? probasbly?
+    requires m0.ownersInKlown(k)
+    requires v.Ready()
+    requires m0.Calid()
+    requires m0.CalidLineKV(k,v)
+    requires k !in m0.m.Keys
+    requires v !in m0.m.Values
+    requires v in  m0.hns({v})
+    requires m1.from(m0)
+    requires m1 == klonKV(m0,k,v)
+     ensures m1.m == vmapKV(m0.m,k,v)
+     ensures k in m1.m.Keys
+     ensures m1.m.Keys   == m0.m.Keys + {k}
+     ensures m1.m.Values == m0.m.Values + {v}
+     ensures m1.m[k] == v
+     ensures m1.objectInKlown(k)
+     ensures m1.Calid()
+//ensures HighCalidFragilistic(m1)
+
+{
+    assert m1 == m0.CalidKV(k,v);
+    assert m1.Calid();
+    //assume m1.Calid();  //still crashes
+}
+
+
+
+
+
+//this costs 0.08ms - who knows whw?
+lemma OIKsisOIKs(o : Object, m : Klon)
+  requires o.Ready()
+  requires m.ownersInKlown(o)
+  ensures forall oo <- o.AMFO | oo != o :: m.ownersInKlown(oo)
+  ensures forall oo <- o.AMFX :: m.ownersInKlown(oo)
+{}
+
+
+////////// shifting
+
+
+function {:isolate_assertions} shiftObject(i0 : Object, m : Klon) : (i1 : Object)
+// see below BETTER version but with stronger preconditions
+// kept this one becuase the necessary refactoring needs to come later //JDl
+    requires m.apoCalidse()
+//    requires m.SuperCalidFragilistic()
+//     ensures m.AllLinesCalid()
+    requires i0.Ready()
+    requires inside(i0, m.o)
+    requires m.objectInKlown(i0)
+
+//    ensures inside(i1, m.m[m.o] )
+    //    reads m.hns()
+    { m.m[i0] }
+
+
+
+
+
+function {:isolate_assertions} shiftAMFO(i0 : OWNR, x0 : OWNR, x1 : OWNR, im : vmap<Object, Object>) : (i1 : OWNR)
+ //given i0 insidfe x0, shift it sideways to the same relationship with w1
+ //fuck - perhaps this needs a Klon.  probalby does!
+ // lemmee guess, this thrns out to b som version of nmapwthKlon.  fucker.  commie FUCK.
+ // except coming in as OWNRs not Owners or Objects
+ //grrr
+ //**wont verify with just apoCalidse..  */
+  requires i0 >= x0
+  requires i0 <= im.Keys
+     //aka requires im.Keys >= i0 >= x0
+   ensures i1 >= x1
+   ensures i1 == (set o <- (i0 - x0) :: im[o]) + x1
+               { (set o <- (i0 - x0) :: im[o]) + x1 }
+
+function {:isolate_assertions} shiftAMFOF(i0 : OWNR, x0 : OWNR, x1 : OWNR, im : vmap<Object, Object>) : (i1 : OWNR)
+ //given i0 insidfe x0, shift it sideways to the same relationship with w1
+ //fuck - perhaps this needs a Klon.  probalby does!
+ // lemmee guess, this thrns out to b som version of nmapwthKlon.  fucker.  commie FUCK.
+ // except coming in as OWNRs not Owners or Objects
+ //grrr
+ //**wont verify with just apoCalidse..  */
+  requires flatten(i0) >= x0
+  requires i0 <= im.Keys
+     //aka requires im.Keys >= i0 >= x0
+   ensures flatten(i1) >= x1
+   ensures i1 == (set o <- (i0 - x0) :: im[o]) + x1
+               { (set o <- (i0 - x0) :: im[o]) + x1 }
+
+
+
+function {:isolate_assertions} shiftAMFOZ(i0 : OWNR, x0 : OWNR, x1 : OWNR, im : vmap<Object, Object>) : (i1 : OWNR)
+ //given i0 insidfe x0, shift it sideways to the same relationship with w1
+ //fuck - perhaps this needs a Klon.  probalby does!
+ // lemmee guess, this thrns out to b som version of nmapwthKlon.  fucker.  commie FUCK.
+ // except coming in as OWNRs not Owners or Objects
+ //grrr
+ //**wont verify with just apoCalidse..  */
+  requires i0 <= im.Keys
+     //aka requires im.Keys >= i0 >= x0
+   ensures i1 == (set o <- (i0 - x0) :: im[o]) + x1
+               { (set o <- (i0 - x0) :: im[o]) + x1 }
+
+
+
+
+
+
+
+
+lemma {:isolate_assertions} SubObjectsGeqViaOWNRs(p0 : Object, w0 : Object, p1 : Object, w1 : Object, m : Klon)
+    requires m.SuperCalidFragilistic()
+    requires m.objectReadyInKlown(p0)
+    requires m.objectReadyInKlown(w0)
+    requires inside3(p0,w0,m.o)
+    requires not(inside(w1, w0)) // careful because we want !>= relation, as against < or <=
+    requires p1.AMFO == shiftAMFO(p0.AMFO, m.o.AMFO, m.m[m.o].AMFO, m.m)
+    requires w1.AMFO == shiftAMFO(w0.AMFO, m.o.AMFO, m.m[m.o].AMFO, m.m)
+     ensures inside3(p1,w1,m.m[m.o])
+{}
+
+
+lemma {:isolate_assertions} SubAMFOsGeq(p0 : OWNR, w0 : OWNR, p1 : OWNR, w1 : OWNR, m : Klon)
+    //p0 and w0 are flattened owners )AMFOs( within pivot x0;  (original)
+    //p1 and w1 are flattened owners )AMFOs( within copivot x1;  (clone)
+    requires m.SuperCalidFragilistic()
+    requires m.m.Keys >= p0 >= w0 >= m.o.AMFO
+  //  requires not( w1 >= w0 ) // careful because we want !>= relation, as against < or <=
+    requires p1 == shiftAMFO(p0, m.o.AMFO, m.m[m.o].AMFO, m.m)
+    requires w1 == shiftAMFO(w0, m.o.AMFO, m.m[m.o].AMFO, m.m)
+
+     ensures m.objectReadyInKlown(m.o)
+     ensures m.m[m.o] in m.m.Values
+     ensures sub(p0,m.o.AMFO) >= sub(w0,m.o.AMFO)
+     ensures sub(p1,m.m[m.o].AMFO) >= sub(w1,m.m[m.o].AMFO)
+     ensures p1 >= w1 >= m.m[m.o].AMFO
+{
+    assert m.SuperCalidFragilistic();
+    assert m.objectReadyInKlown(m.o);
+    assert m.m.Keys >= m.o.AMFO;
+    assert forall oo <- m.o.owner :: (oo in m.m.Keys) && (m.m[oo] in m.m.Values);
+    assert forall oo <- m.o.AMFO :: m.m[oo] in m.m.Values;
+
+    assert m.OwnersLineKV(m.o, m.m[m.o]);
+    assert mappingOwnersThruKlownKV(m.o, m.m[m.o], m);
+
+    assert m.o.Ready();
+    assert forall oo <- m.o.owner :: inside(m.o, oo);
+    assert m.m[m.o].Ready();
+    assert forall oo <- m.m[m.o].owner :: inside(m.m[m.o], oo);
+}
+
+lemma {:isolate_assertions} {:timeLimit 60} IWannaBeFoolish(i0 : Object, m : Klon, i1 : Object)
+ //shiftObject is shiftAMFO is mappingOwnersThruKlownKV
+  requires m.objectReadyInKlown(i0)
+  requires m.SuperCalidFragilistic()
+  requires inside(i0, m.o)
+  requires m.m[i0] == i1 ///'not strong enough  (6 Oct 2025)
+  requires i1.AMFO == shiftAMFO(i0.AMFO, m.o.AMFO, m.m[m.o].AMFO, m.m)
+  requires forall z <- (m.m.Keys)   :: z.Ready()
+  requires forall z <- (m.m.Values) :: z.Ready()
+  requires forall z <- (i0.AMFO)    :: z.Ready()
+  requires forall z <- (i1.AMFO)    :: z.Ready()
+  requires flatten(i0.AMFO) <= m.oHeap
+  requires flatten(i1.AMFO) <= m.hns(i1.AMFO)
+
+   ensures i1 == shiftObject(i0, m)
+   ensures i1.AMFO == shiftAMFO(i0.AMFO, m.o.AMFO, m.m[m.o].AMFO, m.m)
+   ensures mappingOWNRsThruKlownKV(i0.AMFO, i1.AMFO, m)
+   {
+
+   var kk := i0.AMFO;
+   var vv := (mapThruKlon(kk - m.o.AMFO, m) + m.m[m.o].AMFO);
+   assert vv == i1.AMFO;
+
+var si0 := i0.AMFO;
+var sx0 := m.o.AMFO;
+var sx1 := m.m[m.o].AMFO;
+var slm := m.m;
+var si1 := shiftAMFO(i0.AMFO, m.o.AMFO, m.m[m.o].AMFO, m.m);
+assert si1 == (set o <- (si0 - sx0) :: slm[o]) + sx1;
+assert si1 == (set o <- (i0.AMFO - m.o.AMFO) :: m.m[o]) + m.m[m.o].AMFO;
+assert si1 == vv;
+
+assert i1.AMFO == si1;
+
+   }
+
+
+
+
+lemma {:isolate_assertions} ShiftAMFOshiftOWNRs(kk : OWNR, vv : OWNR, m : Klon)
+   //establishes that shiftAMFO(Kk) makes a vv that passes mappignOWNRS...
+      requires m.apoCalidse()
+      requires AllReady(kk)
+      requires AllReady(vv)
+      requires kk <= m.m.Keys
+      requires kk >= m.o.AMFO
+
+      requires flatten(kk) <= m.oHeap
+      requires flatten(vv) <= m.hns(vv)  //kind of trivially true though...
+
+      requires vv == shiftAMFO(kk, m.o.AMFO, m.m[m.o].AMFO, m.m)
+
+       //ensures vv == (mapThruKlon(kk - m.o.AMFO, m) + m.m[m.o].AMFO)
+
+       ensures mappingOWNRsThruKlownKV(kk, shiftAMFO(kk, m.o.AMFO, m.m[m.o].AMFO, m.m), m)
+      {}
+
+
+lemma {:isolate_assertions} ShiftOWNRshiftAMFOs(kk : OWNR, vv : OWNR, m : Klon)
+    //or this? 0 if mappign OWNRS are OK< then shitAMFO doea the righ tthing
+      requires m.apoCalidse()
+      requires AllReady(kk)
+      requires AllReady(vv)
+      requires kk <= m.m.Keys
+
+      requires kk >= m.o.AMFO
+      requires mappingOWNRsThruKlownKV(kk, vv, m)
+      ensures vv == shiftAMFO(kk, m.o.AMFO, m.m[m.o].AMFO, m.m)
+      {}
