Klon-Random.dfy
@@ -1,0 +1,196 @@
+include "Klon-Lemmata.dfy"
+
+lemma {:isolate_assertions} KindaStupid(k : Object, v : Object, m : Klon)
+ //if we're OwnersCalid, and k is in m, then we get stuff
+  requires m.CalidOwners()
+  requires m.HeapOwnersReady() //grrr
+  requires k.Ready() && m.objectInKlown(k)
+  requires v.Ready() && m.objectInKlown(v)
+  requires m.m[k] == v
+   ensures m.OwnersLineKV(k,v)
+   ensures mapThruKlon({k},m) == {v}
+{
+  assert  v  == m.m[k];
+  assert {v} == {m.m[k]};
+  assert {v} == set o <- {k} :: m.m[o];
+  assert {v} == mapThruKlon({k},m);
+}
+
+
+lemma  {:isolate_assertions} {:timeLimit 15} MapThruKlonOutsideOwner(k : Object, m : Klon)
+  requires m.CalidOwners()
+  requires m.HeapOwnersReady() //grrr
+  requires k.Ready() && m.objectInKlown(k)
+  requires outside(k, m.o)
+   ensures mapThruKlon(k.owner, m) == k.owner
+   ensures mapThruKlon(k.bound, m) == k.bound
+{
+  assert outside(k, m.o);
+//  assert forall oo <- k.owner ::  inside(m.o, oo);
+  assert forall oo <- m.m.Keys | outside(oo, m.o) :: m.m[oo] == oo;
+  assert forall oo <- k.owner  | outside(oo, m.o) :: m.m[oo] == oo;
+  assert forall oo <- k.owner  :: outside(oo, m.o);
+  assert forall oo <- k.owner  :: (m.m[oo] == oo);
+  assert (set o <- k.owner :: m.m[o]) == k.owner;
+  assert mapThruKlon(k.owner, m) == k.owner;
+
+  assert forall oo <- k.bound  | outside(oo, m.o) :: m.m[oo] == oo;
+  assert forall oo <- k.bound  :: outside(oo, m.o);
+  assert forall oo <- k.bound  :: (m.m[oo] == oo);
+  assert (set o <- k.bound :: m.m[o]) == k.bound;
+  assert mapThruKlon(k.bound, m) == k.bound;
+}
+
+lemma {:isolate_assertions} NotFromAJedi(k : Object, v : Object, m : Klon)
+  requires m.CalidOwners()
+  requires m.HeapOwnersReady() //grrr
+  requires k.Ready() && m.objectInKlown(k)
+  requires v.Ready() && m.objectInKlown(v)
+  requires m.m[k] == v
+
+  requires mapThruKlon(k.owner, m) == v.owner
+  requires mapThruKlon(k.bound, m) == v.bound
+
+   ensures mapBackKlon(v.owner, m) == k.owner
+   ensures mapBackKlon(v.bound, m) == k.bound
+
+  {
+    ThereAndKlonAgain1(k.owner, m, v.owner);
+    ThereAndKlonAgain1(k.bound, m, v.bound);
+
+   }
+
+
+lemma {:isolate_assertions} OnlyAMasterOfEvilDarth(k : Object, v : Object, m : Klon)
+  //showing how this was previous fucked up
+//BUT YOU FUCKED IT UP -- IT CAN'T!!!!!!!!
+//NOT WHEN k == mn.o at least?
+  requires m.apoCalidse()
+  requires m.CalidOwners()
+  requires m.HeapOwnersReady() //grrr
+  requires k.Ready() && m.objectInKlown(k)
+  requires v.Ready() && m.objectInKlown(v) //WTF?? - this FUCKS EVERYTHING, only vadlid if k outside m.o
+  requires m.m[k] == v
+   ensures m.OwnersLineKV(k,v)
+   ensures mapThruKlon({k},m) == {v}
+
+   ensures outside(k, m.o)  //WHOOPS APOCALYPSE!
+   {}
+
+lemma {:isolate_assertions} OnlyNowAtTheEndDoYouUnderstand(k : Object, v : Object, m : Klon)
+  //wpeoves mapTHruKlon works in all cases of original being inside,outside, eq m.o
+//BUT YOU FUCKED IT UP -- IT CAN'T!!!!!!!!
+//NOT WHEN k == mn.o at least? --
+  requires outside(k, m.o)
+  requires m.apoCalidse()
+  requires m.CalidOwners()
+  requires m.HeapOwnersReady() //grrr
+  requires k.Ready() && m.objectInKlown(k)
+  requires v.Ready() //&& m.objectInKlown(v) //WTF?? - this FUCKS EVERYTHING, only vadlid if k outside m.o
+  requires m.m[k] == v
+   ensures m.OwnersLineKV(k,v)
+   ensures mapThruKlon({k},m) == {v}
+   ensures mapThruKlon(k.owner, m) == v.owner
+   ensures mapThruKlon(k.bound, m) == v.bound
+  {
+    assert m.CalidOwners();
+    assert m.apoCalidse();
+    assert(forall z <- m.m.Keys :: m. OwnersLineKV(z, m.m[z]));
+    assert m.OwnersLineKV(k,v);
+    assert mappingOwnersThruKlownKV(k, v, m);
+
+    assert (k == m.o) || (outside(k, m.o)) || strictlyInside(k, m.o);
+
+    assert (k == m.o)  ==>  not((outside(k, m.o)) || strictlyInside(k, m.o));
+    assert (outside(k, m.o))  ==>  not((k == m.o) || strictlyInside(k, m.o));
+    assert (strictlyInside(k, m.o)) ==> not((outside(k, m.o)) || (k == m.o));
+
+    if (k == m.o) {
+        assert m.m[k] == m.m[m.o] == v;
+        assert (v.owner == m.clowner);
+        assert (v.bound == m.clbound);
+        assert m.m[k].owner == v.owner;
+        assert m.m[k].bound == v.bound;
+
+        // assert mappingOWNRsThruKlownKV(k.owner, v.owner, m);
+        // assert mappingOWNRsThruKlownKV(k.bound, v.bound, m);
+        assert mapThruKlon(k.owner, m) == v.owner;
+        assert mapThruKlon(k.bound, m) == v.bound;
+    }
+
+    if (outside(k, m.o)) {
+        assert m.m[k] == v;
+        assert k == v;
+        assert m.m[k] == k;
+        assert k.owner == m.m[k].owner == v.owner;
+        assert k.bound == m.m[k].bound == v.bound;
+
+        assert not( mappingOWNRsThruKlownKV(k.owner, v.owner, m) );
+        assert not( mappingOWNRsThruKlownKV(k.bound, v.bound, m) );
+
+        MapThruKlonOutsideOwner(k, m);
+        assert  mapThruKlon(k.owner, m) == k.owner == v.owner;
+        assert  mapThruKlon(k.bound, m) == k.bound == v.bound;
+    }
+
+    if (strictlyInside(k, m.o)) {
+        assert k != v;
+        assert m.m[k] == v;
+        assert m.m[k].owner == v.owner;
+        assert m.m[k].bound == v.bound;
+
+        assert mappingOWNRsThruKlownKV(k.owner, v.owner, m);
+        assert mappingOWNRsThruKlownKV(k.bound, v.bound, m);
+        assert mapThruKlon(k.owner, m) == v.owner;
+        assert mapThruKlon(k.bound, m) == v.bound;
+    }
+
+    assert mapThruKlon(k.owner, m) == v.owner;
+    assert mapThruKlon(k.bound, m) == v.bound;
+
+    KindaStupid(k,v,m);
+    assert mapThruKlon({k},m) == {v};
+}
+
+
+
+
+
+
+
+
+
+
+
+
+
+
+
+predicate {:isolate_assertions} OLDcheckBoundOfClone(k : Object, v : Object, m : Klon)
+  //to work, this needs m.o and m.m[m.o] to be set up
+  //but does NOT need k in Keys, or v in values!
+  //
+  // apparently doesn't even need Caliud or precalid let alone supercalid.  HMMM
+  requires k.Ready()
+  requires m.ownersInKlown(k)
+  requires v.Ready()
+
+
+  //the six requirements of preCalid2 / computeOwnerForClone apocalypse
+  requires k.owner <= m.m.Keys <= m.oHeap
+  requires m.m.Values <= flatten( m.hns() )
+  requires m.o.Ready()
+  requires m.objectInKlown(m.o)
+  requires m.HeapOwnersReady()
+  requires m.c_amfx <= m.oHeap
+  reads {}
+{
+  || (v == k)   //note technically redundant condition...
+  || (v.AMFB >=  k.AMFB)  //GREENLAND //Beady2()  //AMFB_GEQ_GT
+     //when you clone you can *(either)*
+      //move the owner down
+      //move the bound down (allowing more pointing but less movement)
+      //move the owner up to the bound
+       //providing you don't break any other invariant...
+      // you do need to be able to "copy out" and "copy in"
+}
