Klon.dfy
@@ -1,0 +1,1547 @@
+include "Ownership.dfy"
+
+
+// //[[[[[[[[[[[[[[[[[[[[[[[[[[[[[[[[[[[[[[[[]]]]]]]]]]]]]]]]]]]]]]]]]]]]]]]]]]]]]]]]
+// //[[[[[[[[[[[[[[[[[[[[[[[[[[[[[[[[[[[[[[[[]]]]]]]]]]]]]]]]]]]]]]]]]]]]]]]]]]]]]]]]
+// //
+// //  Klon - clone mapping!
+// //
+// //[[[[[[[[[[[[[[[[[[[[[[[[[[[[[[[[[[[[[[[[]]]]]]]]]]]]]]]]]]]]]]]]]]]]]]]]]]]]]]]]
+// //[[[[[[[[[[[[[[[[[[[[[[[[[[[[[[[[[[[[[[[[]]]]]]]]]]]]]]]]]]]]]]]]]]]]]]]]]]]]]]]]
+//
+//
+//
+//  thinkgs to add - the two level version?  (PreKlon and Klon?)
+//    c - : objecet --=- the top of the clone! hurrah! m.m[m.o]!
+
+datatype Klon = Klon
+(
+  m : vmap<Object,Object>,    //the  klon map
+  o : Object,                 //object being copied
+  clowner : Owner,            //owner of the clone
+  clbound : Owner,            //bound of the clone
+  oHeap : set<Object>,        //heap
+  o_amfx : Owner,             //was o. so the AMFX of o
+  //  c_amfb : OWNR,              //epected flattened bound of the clone..
+  c_amfx : Owner              //epected flattened ownershio of the clone..
+)
+{
+  function  ns(os : set<Object> := {}) : set<Object> { m.Values+os        }
+  function hns(os : set<Object> := {}) : set<Object> { oHeap+m.Values+os  }
+
+  predicate from(prev : Klon) : (r : bool)
+    ensures r ==> (isFlat(prev.oHeap) ==> isFlat(oHeap))
+  {
+    && mapGEQ(m,  prev.m)
+    && o       == prev.o
+    && clowner == prev.clowner
+    && clbound == prev.clbound
+    && oHeap   == prev.oHeap     //OPTION - considere incorporating ApoCalidseNow...
+    && o_amfx  == prev.o_amfx
+    && c_amfx  == prev.c_amfx
+       //option ie allow heaps to get bigger, so long as all keys are in the heap
+  }
+
+
+  predicate HeapOwnersReady()
+    reads {}
+  { forall x <- oHeap :: (x.AMFO <= oHeap) }
+
+  predicate ValuesOwnersReady()
+    reads {}
+  {
+   forall x <- m.Values :: (x.AMFO <= hns())
+  }
+
+  predicate HeapContextReady()
+    reads oHeap
+  {///KJX 1 Augu 2025 - not sure this is right cos
+   ///do3esentt that contradict the heap p      ointoting to na
+   ///i.e. heap ispart of hns isn't it?
+   ///answer yes, but that doen't happen during a clone() operation...
+    (forall x <- oHeap :: (x.Ready() && x.Valid() && x.Context(oHeap)))
+  }
+
+  predicate ValuesContextReady()
+    reads m.Values, oHeap
+  {
+    //KJX experimental!! 11 aug 2025
+   forall x <- m.Values :: x.Context(hns())  ///KJX HACKED 4 Oct 2025    ///shojld this say "READY"
+  //or should this be hns too?
+//    (forall x <- m.Values :: (x.Ready() && x.Valid() && x.Context(hns())))
+  }
+
+predicate ValueInContext(v : Object)
+  requires ValuesContextReady()   //WHAT THE FUYCK???
+  requires v in hns()
+  reads hns(),  m.Values, oHeap
+  { (v.Ready() && v.Valid() && v.Context(hns())) }
+
+
+
+  ghost predicate {:isolate_assertions}   preCalid() : (r : bool)
+    //Klon mapping is consitent & valid.
+    //Calid just seened like a good name
+    reads oHeap, m.Values
+
+    // requires HeapContextReady()
+    // requires ValuesContextReady()
+  {
+    //internal consistency
+    //note that the pivot object being clone "o"
+    //does not hace to be in the map at the start.
+
+    //&& (isFlat(oHeap))  //KJXFEARSATAN
+
+    && HeapContextReady()
+    && ValuesContextReady()
+
+    && (o in oHeap)
+    && (objectInKlown(o))  //KJXFUCK  do i want this in here? really?   ///Can U do without it??
+    && (o.AMFX == o_amfx)
+//WTF    && (flatten(clbound) >= o.AMFB)
+    && (nuBoundsOK(o.owner, o.bound))
+    && (o.AMFO == o_amfx+{o})
+   //bound can only move DOWN
+    //    && (not(c_amfx > o_amfx)) //HUMBERT HUMBERT
+    // important to note that c_amfx can be any distance below o_amfx -
+    // or more accurately, any distance below o.bound
+    // which may (or may not) be *above*/*outside* o_amfx.
+    && (c_amfx >= flatten(clbound) >= flatten(o.bound))
+  }
+
+
+
+  ghost predicate {:isolate_assertions} preCalid2() : (r : bool)
+    //More PreCalid2 Stuff
+    // reads oHeap`fields, oHeap`fieldModes
+    // reads m.Keys`fields, m.Keys`fieldModes
+    // reads m.Values`fields, m.Values`fieldModes
+    // reads o`fields, o`fieldModes
+    // reads m.Values, oHeap
+
+    reads {}
+  {
+    //   m : vmap<Object,Object>,    //the  klon map
+    //   o : Object,                 //object being copied
+    //   clowner : Owner,            //owner of the clone
+    //   clbound : Owner,            //bound of the clone
+    //   oHeap : set<Object>,        //heap
+    //   o_amfx : Owner,             //was o. so the AMFX of o
+    // //  c_amfb : OWNR,              //epected flattened bound of the clone..
+    //   c_amfx : Owner
+
+    && (c_amfx <= oHeap) //should goto precalid1??
+      //Llooks kinda odd...
+
+    && ((o in m.Keys) ==> (
+        var c := m[o]; //WE HAS KLONE
+         ///&& add in c.Ready()???
+          && (c_amfx  == c.AMFX)
+          && (clowner == c.owner)
+          && (clbound == c.bound)
+
+          && (c  in m.Values)
+          && (c !in oHeap)
+       ))
+  }
+
+  ghost predicate {:isolate_assertions} SuperCalidFragilistic() : (r : bool)
+    //Klon mapping is consitent & valid.
+    //Calid just seened like a good name
+
+    reads oHeap, m.Values
+///can goto reads {} bia HeapOwnersReady && ValuesOwnersReady…
+
+    // reads oHeap`fields, oHeap`fieldModes
+    // reads m.Keys`fields, m.Keys`fieldModes
+    // reads m.Values`fields, m.Values`fieldModes
+    // reads o`fields, o`fieldModese
+    // reads m.Values, oHeap
+  {
+//    false  //WHAT THE FUCKY FUCK FUCK???4
+    && HeapContextReady()
+    && ValuesContextReady()
+    && Calid()
+  }
+
+  //opaque
+  ghost predicate {:isolate_assertions} Calid() : (r : bool)
+    //Klon mapping is consitent & valid.
+    //Calid just seened like a good name
+
+    //dont call this directly - call SuperCalid
+    requires  HeapContextReady()
+    requires  ValuesContextReady()
+
+    reads oHeap, m.Values
+ {
+    //internal consistency
+    && preCalid()
+    && preCalid2()
+
+    //calidObjects - mostly about oHeap and ns and stuff
+    && (m.Keys <= oHeap)
+    && (forall k <- m.Keys :: (k.Ready() && k.Valid()))   //note no Context
+
+    //this recapitulates ValuesContextReady() but putting it here lets things work
+    && (forall v <- m.Values :: (v.Ready() && v.Valid()))    //note no Context
+
+    //the pivot object "o" being cloned
+    // && (o.Ready() && o.Valid() && o.Context(oHeap) && objectInKlown(o))
+    && (o.Ready() && o.Valid() && o.Context(oHeap) && objectInKlown(o))
+
+    //what's all this SHIT and why is it here and how doe it realte to allLinesCallid etc!
+    && (forall k <- m.Keys   :: m[k].AMFO  >= m[k].AMFB  >= k.AMFB)
+//      && (forall k <- m.Keys   :: m[k].AMFO  >= m[k].AMFB >= o.AMFB >= k.AMFB)   ///change made then backed out 10Jul 2025 - why wo why oh why ?
+
+    // && (forall k <- m.Keys   :: m[k].owner >= m[k].bound >= k.bound)
+    && (forall k <- m.Keys   :: (not(inside(k,o)) ==> (m[k] == k)))
+    && (forall k <- m.Keys   :: (   (inside(k,o)) ==> (m[k] !in oHeap)))
+    //
+    //calidSheep - su WRONGbsumed?
+    //12 Jine 2025 clipping this out for now
+
+    //KlonVMqpOK(k, context)
+    && (forall k <- m.Keys :: k.AMFO <= m.Keys)
+    && (forall k <- m.Keys :: k.AMFB <= m.Keys)
+
+    && (&& (HeapOwnersReady())
+        //  && ((forall x <- m.Keys :: x.Ready() && x.Valid() && x.Context(oHeap) && objectInKlown(x)   ))
+        && (ValuesOwnersReady())
+        && (gettingThere())
+        && (AllLinesCalid()))
+
+    //    && (forall k <- m.Keys :: ownersInKlown(k) && checkClownership(k, m[k], this))
+  }
+
+
+
+//   //removeing the var declaratioon on this end
+//   //made things work on the other!
+  predicate gettingThere() reads {} {
+    // forall k <- m.Keys ::
+    //     (var v := m[k];
+    //     && (k.Ready())
+    //     && (objectInKlown(k))
+    //     && (v.Ready())
+    //     && (v in hns({v})))
+    forall k <- m.Keys :: (
+                            && (k.Ready())
+                            && (objectInKlown(k))
+                            && (m[k].Ready())
+                            && (m[k] in hns())
+                          )
+
+  }
+
+//
+//   //and again --- isses are things like HeapContexReady, ValuesContext, reqs vs conjuncts,
+  predicate {:isolate_assertions} AllLinesCalid()
+    //all pairs (aka lines) in the overall Klon map are Calid
+    requires gettingThere()
+
+    requires o.Ready() && objectInKlown(o)
+    requires m.Keys <= oHeap
+
+    //what's left of the six requirements of preCalid2 / computeOwnerForClone apocalypse
+    requires HeapOwnersReady()
+    requires c_amfx <= oHeap
+    reads oHeap, m.Values
+  {
+    (forall k <- m.Keys :: CalidLineKV(k, m[k]))
+  }
+
+//
+//
+//
+//
+//
+
+  lemma {:isolate_assertions} {:timeLimit 20} CalidLineKVTo(k : Object, v : Object, m1 : Klon)
+    requires apoCalidse()
+    requires k.Ready()// && k.Valid() // should context go in here too? probasbly?
+    requires ownersInKlown(k)
+    requires v.Ready()
+    requires CalidLineKV(k,v)
+    requires m1.from(this)
+    requires m1.apoCalidse()
+     ensures m1.CalidLineKV(k,v)
+{}
+
+
+  predicate {:isolate_assertions} CalidLineKV(k : Object, v : Object)
+    //conditions for individual mappings (pairs aka lines) in the overall Klon map
+    //this shoiuld work for lines *already* in the Klon
+    //*as well as* for lines that aren't into the Klon
+    ///(but it won't tell you if you can add them cos they could be already in there)
+    requires apoCalidse()
+    requires k.Ready()// && k.Valid() // should context go in here too? probasbly?
+    requires ownersInKlown(k)
+    requires v.Ready()
+
+    reads oHeap, m.Values
+  {
+
+    && (k in oHeap)    //this one is easy - what to do for things like v.AMFO aren't...
+    //or perhaps it is - they either ibn the preheap or ns newstuff
+        //KJX - 10 Aug 2025
+
+    //the fundamental something-or-other
+    && (not(inside(k,o)) ==> (v == k))
+    && (   (inside(k,o)) ==> (v !in oHeap))
+//    && (   (inside(k,o)) ==> (v.AMFO  >= v.AMFB >= k.AMFB))  //Beady2() GREENLAND
+    && (   (inside(k,o)) ==> (k.AMFB <= o.AMFB) )  // GREENLAND
+      ////Beady2()  GREENLAND -
+  //    && (   (inside(k,o)) ==> (v.owner >= v.bound >= k.bound >= o.bound))
+
+//    && ( (v.AMFO > v.AMFB  >= k.AMFB) )   //GREENLAND
+
+//  && ( (v.owner >= v.bound >= k.bound) )
+
+    && (k.AMFX <= m.Keys)
+    && (k.AMFB <= m.Keys)
+//    && (k.bound <= k.owner <= m.Keys)
+    && (ownersInKlown(k))  //belt and braces--- currently a requirement!
+    && (checkOwnershipOfClone(k,v,this))
+    && (checkBoundOfClone(k,v,this))
+
+  //MAPPING - KJXFEARSATAN
+    && (mappingOwnersThruKlownKV(k,v,this))
+
+///k.fieldModes == v.fieldModes  ///or shoudl otherwise be compatible
+
+  }
+
+lemma MOVIN_ON_MAP(os: Owner, left : vmap<Object,Object>, right : vmap<Object,Object>)
+  requires left.Keys >= right.Keys >= os
+  requires forall o <- right.Keys :: left[o] == right[o]
+  ensures  (set o <- os :: left[o]) == (set o <- os :: right[o])
+{}
+
+
+
+  predicate objectInKlown(o : Object) : (rv : bool)
+    //o and all its owners etc are the Klown m
+    //(doesn't extend to fields)
+    //BUT should incorproate ready!! like ObjectReadyInKlon - merge these in
+    reads {}
+    requires o.Ready()
+
+    ensures rv ==> (o in m.Keys)
+    ensures rv ==> (o.AMFB <= m.Keys)
+    ensures rv ==> (o.AMFX <= m.Keys)
+    ensures rv ==> (o.AMFO <= m.Keys)    //WEESA DONT WANTA REQUIRE this MASSA
+    ensures rv ==> (o.bound <= m.Keys)
+    ensures rv ==> (o.owner <= m.Keys)
+    ensures rv ==> (o.self  <= m.Keys)    //WEESA DONT WANTA REQUIRE this MASSA
+  { o.AMFO <= m.Keys }
+
+
+  predicate ownersInKlown(o : Object) : (rv : bool)
+    //o's owners but not o itself is in the Klon
+    //(doesn't extend to fields)
+    reads {}
+
+    //critical that thes does *not* catch AMFO or self ...
+    requires o.Ready()
+
+    ensures rv ==> (o.AMFB <= m.Keys)
+    ensures rv ==> (o.AMFX <= m.Keys)
+    ensures rv ==> (o.bound <= m.Keys)
+    ensures rv ==> (o.owner <= m.Keys)
+  { o.AMFX <= m.Keys }
+
+  predicate objectReadyInKlown(o : Object) : (rv : bool)
+    //o and all its owners etc are the Klown m
+    //(doesn't extend to fields)
+    reads {}
+
+    ensures rv ==> (o in m.Keys)
+    ensures rv ==> (o.AMFB <= m.Keys)
+    ensures rv ==> (o.AMFX <= m.Keys)
+    ensures rv ==> (o.AMFO <= m.Keys)
+    ensures rv ==> (o.bound <= m.Keys)
+    ensures rv ==> (o.owner <= m.Keys)
+    ensures rv ==> (o.self  <= m.Keys)
+
+    ensures (o.Ready() && rv) ==> objectInKlown(o)
+    ensures  o.Ready() ==> (rv == objectInKlown(o))
+
+  {
+    o.Ready() && (o.AMFO <= m.Keys)
+   }
+
+  predicate ownersReadyInKlown(o : Object) : (rv : bool)
+    ensures rv ==> (o.AMFB <= m.Keys)
+    ensures rv ==> (o.AMFX <= m.Keys)
+    ensures rv ==> (o.bound <= m.Keys)
+    ensures rv ==> (o.owner <= m.Keys)
+    ensures rv ==> (o.Ready())
+
+    ensures (o.Ready() && rv) ==> ownersInKlown(o)
+    ensures  o.Ready() ==> (rv == ownersInKlown(o))
+
+    reads {}
+    {
+      o.Ready() && (o.AMFX <= m.Keys)
+    }
+
+//29 Oct 2025
+//I think the quesiton is whether clowner have tio be in values.
+//and ... it doesn't!!!
+  // lemma ObjectValuesInKlownToo(o : O bject)
+  //   requires objectInKlown(o)
+  //   requires CalidOwners()
+  //    ensures m[o].AMFO <= m.Values
+  //       {
+  //           assert o.AMFO <= n.Keys; requires f.AMFO >= t.AMFX   ///classic O-as-D, f->t ==> f inside T.owner
+  //           assert forall x <- o.AMFO :: CalidLineKV(x, m[x]);
+  //       }
+
+
+predicate  apoCalidse()
+   //the six requirements of preCalid2 / computeOwnerForClone apocalypse
+   reads {}
+  {
+    && (m.Keys <= oHeap)
+    && (m.Values <= hns())
+    && (objectReadyInKlown(o))   //this was originally two predicates
+    && (HeapOwnersReady())  //whatt bno value owners ready??
+    && (c_amfx <= oHeap)
+  }
+
+//{:timeLimit 60}
+  function {:isolate_assertions} {:timeLimit 30} CalidKV(k : Object, v : Object) : (mK : Klon)
+    //givne a Calid Klon, add in k:=v to the mapping and get a  Calid result.
+    //the heart of the heart of the klon
+
+    requires CKV_preconditions(k,v)
+    requires CalidLineKV(k,v)    requires CLKV: CalidLineKV(k,v)
+
+     ensures mK == klonKV(this, k, v)
+     ensures mK.from(this)
+     ensures mK.HeapContextReady()
+     ensures mK.ValuesContextReady()
+     ensures mK.m.Keys <= mK.oHeap
+     // ensures  unchanged(oHeap`fieldModes)
+     // ensures  unchanged(m.Values`fieldModes)
+     ensures forall z <- m.Keys :: m[z].fieldModes == mK.m[z].fieldModes
+
+     ensures mK.Calid()
+     ensures mK.SuperCalidFragilistic()
+
+     reads oHeap, m.Values, k, v
+     reads m.Keys, m.Values
+  {
+       assert CKV_preconditions(k,v);
+    // assert CKV_preconditions(k,v);
+    //
+    //----------------------------------------------------------------------
+    //
+    // assert SuperCalidFragilistic();
+    // assert k.Ready();
+    // assert ownersInKlown(k);
+    // assert o.Ready();
+    // assert objectInKlown(o);
+    // assert CalidCanKey(k);
+    // assert k !in m.Keys;
+    // assert v !in m.Values;
+    // assert HeapContextReady();
+    // assert ValuesContextReady();
+    // assert Calid();
+    // assert k in oHeap;
+    // assert (v.Ready() && v.Context(hns({v})));
+    // assert this.m.Keys <= this.oHeap;
+    // assert klonVMapOK(m);
+    // assert klonCanKV(this, k, v);
+    // assert CalidLineKV(k,v);
+    //
+    //
+    //     requires SuperCalidFragilistic()
+    //
+    //     requires k.Ready() //&& k.Valid() // should context go in here too? probasbly?
+    //     requires ownersInKlown(k)   //be nice to get rid of this...
+    //     requires o.Ready() //&& o.Valid()
+    //     requires objectInKlown(o)
+    //
+    //     requires CalidCanKey(k)
+    //
+    //     requires k !in m.Keys
+    //     requires v !in m.Values
+    //
+    //     // requires HeapContextReady()
+    //     // requires ValuesContextReady()
+    //     // requires Calid()
+    //
+    //     requires k in oHeap
+    //     requires (v.Ready() && v.Context(hns({v})))
+    //
+    //     requires this.m.Keys <= this.oHeap
+    //
+    //     requires klonVMapOK(m)
+    //     requires klonCanKV(this, k, v)
+    //
+    //     requires CalidLineKV(k,v)
+    //
+    //----------------------------------------------------------------------
+//
+//
+//     assert preCalid();
+//     assert preCalid2();
+//     assert && (c_amfx <= oHeap);
+//
+//     assert HeapContextReady();
+//
+//     assert forall x <- m.Keys :: (x.Ready() && objectInKlown(x))
+//       by { assert SuperCalidFragilistic(); }        // SuperCalidGetsAllOwnersReadyInKlown();\\
+//
+//     assert ValuesContextReady();
+//     assert AllLinesCalid();
+//
+//
+//     //use kalidLineKV rather than checkOwnershipOfClone(k, m[k], this);
+//     //assert forall k <- m.Keys :: checkOwnershipOfClone(k, m[k], this);
+//
+  (
+     var mK := klonKV(this, k, v);
+     assert mK.m[k] == v;
+
+     assert mK.m.Keys            == m.Keys+{k};
+     assert mKmVmVv: mK.m.Values == m.Values+{v};
+     assert          mK.m.Values == m.Values+{v};
+     assert mK.from(this);
+
+     assert hns({v}) == mK.hns({});
+     assert v.Context(hns({v})) by { assert CKV_preconditions(k,v); }
+     assert v.Context(mK.hns({}));
+
+     forall x <- mK.m.Keys ensures {:contradiction} (mK.m.Keys <= oHeap) //by
+     {
+       if (x == k) { assert {:contradiction} k in oHeap; }
+       if (x != k) { assert {:contradiction} x in oHeap; }
+       assert {:contradiction} x in oHeap;
+     }
+
+     forall y <- mK.m.Values ensures (y.Context(mK.hns())) //by
+     {
+       if (y == v) { assert v.Context(mK.hns()); }
+       if (y != v) {
+         assert  {:contradiction} y in m.Values;
+         assert  {:contradiction} y.Context(hns());
+                                  y.WiderContext(hns(), mK.hns());
+         assert  {:contradiction} y.Context(mK.hns()); }
+
+     }
+
+    //  forall y <- mK.m.Values ensures (y.Ready() && y.Valid() ) //by
+    //  {
+    //    if (y == v) { assert (v.Ready() && v.Valid()); }
+    //    if (y != v) {
+    //      assert  {:contradiction} y in mK.m.Values;
+    //      assert  {:contradiction}  (y.Ready() && y.Valid()); }
+    //  }
+
+
+
+     assert {:contradiction} mK.HeapContextReady();
+     assert ValuesContextReady();
+
+     assert  forall x <- m.Values :: x.OwnersWithin(hns());
+         // assert  (forall x <- m.Values :: (x.Ready() && x.Valid() && x.Context(hns())));
+
+     assert v in mK.m.Values;
+    //  assert v.Context(hns({v})) by { assert CKV_preconditions(k,v); }
+     assert v.Context(mK.hns({}));
+     assert mK.m.Values == m.Values + {v};
+
+     assert forall x  : Object <-    m.Values + {v} :: x.OwnersWithin(hns({v}));
+     assert forall x  : Object <- mK.m.Values       :: x.OwnersWithin(mK.hns());
+//     assert mK.ValuesContextReady();
+
+//      assert objectInKlown(o);
+//      assert mK.objectInKlown(o);
+//
+//      assert CalidCanKey(k); //pro you're like to want to walk.
+//      // ^-- no idea what that comment means but…
+//   //seems a but fyckiung late for this level of quibling now!
+// //     assert forall k <- m.Keys :: CalidLineKV(k,v);
+//
+//      assert mK.m.Keys == m.Keys + {k};
+//     //
+//     //  assert forall k <- mK.m.Keys :: mK.objectInKlown(k);
+//
+
+     assert CKV_preconditions(k,v);
+     assert AllLinesCalid();
+     assert forall x <- m.Keys :: CalidLineKV(x,m[x]);
+     assert CalidLineKV(k,v); //GNT by { reveal CLKV; }
+     assert mK.m[k] == v;
+     CalidLineKVTo(k,mK.m[k],mK);
+     assert mK.CalidLineKV(k,v);
+     assert mK.CalidLineKV(k,mK.m[k]);
+//
+//      forall x <- m.Keys ensures ( this.CalidLineKV(x,m[x]) && ( mK.CalidLineKV(x,m[x])))
+// {
+//        assert CalidLineKV(x,m[x]);
+//         //CUL  CalidLineKVKV(mK,x,this);  //wasKVDFrom!!!!Q
+//
+//        // assert x in mK.m.Keys;
+//        // assert mK.m[x] == m[x];
+//        // assert checkOwnershipOfClone(k,v,this);
+//        //      CheckOwnershipOfCloneFrom(k, v, mK, this);
+//        //      computeOwnerForCloneFrom(k, mK, th is);
+//        // CalidlineFrom(mK,x,this);
+//        //      assert checkOwnershipOfClone(k,v,mK);
+//        assert mK.CalidLineKV(x,m[x]);
+//       //
+//       //  assert KCLX: mK.CalidLineKV(x,m[x]);
+//       //  assert       mK.CalidLineKV(x,m[x]) by { reveal KCLX; }
+//       //  assert (this.CalidLineKV(x,m[x]) && mK.CalidLineKV(x,m[x])) by { reveal TCLX, KCLX; }
+// }
+//
+     forall x <- mK.m.Keys ensures mK.CalidLineKV(x,mK.m[x]) //by
+     {
+//       assert CalidLineKV(x, mK.  m[x]);   //how long?  whu knows
+       if (x in m.Keys) {
+         assert mK.m[x] == m[x];
+         assert this.CalidLineKV(x,m[x]);
+         assert x in mK.m.Keys;
+         assert CalidLineKV(x,mK.m[x]);   //how long?  whu knows?
+         CalidLineKVTo(x,mK.m[x],mK);
+         assert mK.CalidLineKV(x,mK.m[x]);
+       } else {
+         assert x == k;
+         assert mK.m[k] == v;
+         assert CalidLineKV(k,v); //GNT by { reveal CLKV; } by { reveal CLKV; }
+         assert this.CalidLineKV(x,mK.m[x]);
+         assert mK.CalidLineKV(x,mK.m[x]);
+       }
+     }
+
+//      assert (forall k <- mK.m.Keys ::  (k.Ready()));
+//      assert (forall k <- mK.m.Keys ::  (mK.objectInKlown(k)));
+//      assert (forall k <- mK.m.Keys ::  (var v := mK.m[k]; (v.Ready())));
+//      assert (forall k <- mK.m.Keys ::  (var v := mK.m[k]; (v in mK.hns({v}))));
+//
+//     //  assert mK.thettinGhere();
+//     //  assert mK.gettingThere();
+//      assert mK.o.Ready();
+//      assert mK.objectInKlown(mK.o);
+//      assert mK.m.Keys <= mK.oHeap;
+//      assert mK.HeapOwnersReady();
+//      assert mK.c_amfx <= mK.oHeap;
+//
+//      assert   (forall k <- mK.m.Keys ::  mK.CalidLineKV(k,m[k]));
+//
+//      assert mK.AllLinesCalid();
+//
+//AND THEN IT ALL GETS SIUPER-WEIrD??
+//
+//      assert (forall k <- mK.m.Keys  ::
+//                (var v := mK.m[k];  var o := mK.o;
+//                                    && (v.Ready())));
+//
+//      assert forall o <- mK.m.Values :: o.Ready() ==> ((o.AMFO >= o.AMFB));
+//
+//      assert (forall k <- mK.m.Keys  ::
+//                (var v := mK.m[k];  var o := mK.o;
+//                                    && (v.Ready())
+//                                    && (v.AMFO >= v.AMFB)
+//                ));
+//
+//      assert (forall k <- mK.m.Keys  ::
+//                (var v := mK.m[k];  var o := mK.o;
+//                                    && (mK.CalidLineKV(k,v))
+//                                    && (not(inside(k,o)) ==> (k == mK.m[k] == v))
+//                 // && (not(inside(k,o)) ==> (v.AMFB == k.AMFB))
+//                 // && (not(inside(k,o)) ==> (v.AMFO >= v.AMFB == k.AMFB))
+//                ));
+//
+//
+//
+//      assert (forall k <- mK.m.Keys  ::
+//                (var v := mK.m[k];  var o := mK.o;
+//                                    && (mK.CalidLineKV(k,v))
+//                                    && (not(inside(k,o)) ==> (k == mK.m[k] == v))
+//                                    && (not(inside(k,o)) ==> (v.AMFB == k.AMFB))
+//                 // && (not(inside(k,o)) ==> (v.AMFO >= v.AMFB == k.AMFB))
+//                ));
+//
+//      assert (forall k <- mK.m.Keys  ::
+//                (var v := mK.m[k];  var o := mK.o;
+//                                    && (mK.CalidLineKV(k,v))
+//                                    && (not(inside(k,o)) ==> (k == mK.m[k] == v))
+//                                    && (not(inside(k,o)) ==> (v.AMFB == k.AMFB))
+//                                    && (not(inside(k,o)) ==> (v.AMFO >= v.AMFB == k.AMFB))
+//                ));
+//
+//
+//
+//      assert (forall k <- mK.m.Keys  ::
+//                (var v := mK.m[k];  var o := mK.o;
+//                                    && (v.Ready())
+//                                    && (v.AMFO >= v.AMFB)
+//                                    && (not(inside(k,o)) ==> (k == mK.m[k] == v))
+//                 // && (not(inside(k,o)) ==> (v.AMFO >= v.AMFB == k.AMFB))
+//                 // && (   (inside(k,o)) ==> (v.AMFO >= v.AMFB >= k.AMFB >= o.AMFB))   ///from CalidLineKV
+//                 // && (   (inside(k,o)) ==> (v.`owner >= v.bound >= k.bound >= o.bound) )
+//                 // && (  mK.m[k].AMFO >= mK.m[k].AMFB >= k.AMFB  )  /// current - early Jun 2025 defiunition from Calid() which soiuld be refacgored
+//                ));
+//
+//      // ///////////////////////////////////////////////////////////////////////////
+//
+//      // ///////////////////////////////////////////////////////////////////////////
+//
+//      assert  (forall k <- mK.m.Keys   :: mK.m[k].AMFO >= mK.m[k].AMFB >= k.AMFB) ;
+//
+// ///assume  (forall k <- mK.m.Keys   :: mK.m[k].AMFO >= mK.m[k].AMFB >= k.AMFB) ;   //WHAT THE FUCK IS THIS DOING HERE
+//
+//      assert mK.HeapContextReady();
+//      assert mK.ValuesContextReady();
+//      // ///////////////////////////////////////////////////////////////////////////
+//      //tryna get calid
+//      assert (mK.Calid())
+//      by {
+//        assert      && mK.preCalid()
+//                    && mK.preCalid2()
+//
+//                    //calidObjects - mostly about oHeap and ns and stuff
+//                    && (mK.m.Keys <= mK.oHeap)
+//                    && (forall k <- mK.m.Keys :: (k.Ready() && k.Valid()))
+//
+//                    //this recapitulates ValuesContextReady() but putting it here lets things work
+//                    && (forall v <- mK.m.Values :: (v.Ready() && v.Valid()))
+//
+//                    //the pivot object "o" being cloned
+//                    // && (o.Ready() && o.Valid() && o.Context(oHeap) && objectInKlown(o))
+//                    && (mK.o.Ready() && mK.o.Valid() && mK.o.Context(mK.oHeap) && mK.objectInKlown(mK.o))
+//
+//                    && (forall k <- mK.m.Keys   :: mK.m[k].AMFO  >= mK.m[k].AMFB  >= k.AMFB)
+// //wont veruify     && (forall k <- mK.m.Keys   :: mK.m[k].AMFO  >= mK.m[k].AMFB  >= mK.o.AMFB >= k.AMFB)    ///change made then backed out  10JKul 2025 - why wo why oh why ?
+// //  WRONG                 && (forall k <- mK.m.Keys   :: mK.m[k].owner >= mK.m[k].bound >= k.bound)
+//
+//                    && (forall k <- mK.m.Keys   :: (not(inside(k,mK.o)) ==> (mK.m[k] == k)))
+//                    && (forall k <- mK.m.Keys   :: (   (inside(k,mK.o)) ==> (mK.m[k] !in mK.oHeap)))
+//                    //
+//                    //calidSheep - su WRONGbsumed?
+//                    //
+//                    //see rant aove...
+//                    //
+//                    //&& (forall k <- mK.m.Keys :: k.fieldModes == mK.m[k].fieldModes)
+//                    //
+//                    //
+//
+//                    //KlonVMqpOK(k, context)
+//                    && (forall k <- mK.m.Keys :: k.AMFO <= mK.m.Keys)
+//                    && (forall k <- mK.m.Keys :: k.AMFB <= mK.m.Keys)
+// //                   && (forall k <- mK.m.Keys :: k.bound <= k.owner <= mK.m.Keys)
+//                    // && (forall k <- m.Keys :: //;this is s"gettingThere" so why twice?
+//                    //      (var v := m[k];
+//                    //         && (k.Ready())
+//                    //         && (objectInKlown(k))
+//                    //         && (v.Ready())
+//                    //         && (v in hns())))
+//
+//                    && (&& (mK.HeapOwnersReady())
+//                        && (mK.ValuesOwnersReady())
+//                        && (mK.gettingThere())
+//                        && (mK.AllLinesCalid()));
+//      } //tryna
+//
+     assert mK.Calid();
+     assert mK.SuperCalidFragilistic();
+     mK
+  )
+
+}
+//end CalidKV
+
+
+
+
+  ghost predicate {:isolate_assertions} CKV_preconditions(k : Object, v : Object)
+    //attempt to capture the common preconditions for CalidKV
+
+    reads oHeap, m.Values, k, v
+    reads m.Keys, m.Values
+  {
+    && SuperCalidFragilistic()
+
+    && k.Ready() //&& k.Valid() // should context go in here too? probasbly?
+    && ownersInKlown(k)   //be nice to get rid of this...
+    && o.Ready() //&& o.Valid()
+    && objectInKlown(o)
+
+    && CalidCanKey(k)
+
+    && k !in m.Keys
+    && v !in m.Values
+
+    // && HeapContextReady()
+    // && ValuesContextReady()
+    // && Calid()
+
+    && k in oHeap
+    && (v.Ready() && v.Valid() && v.Context(hns({v})))
+
+    && this.m.Keys <= this.oHeap
+
+    && klonVMapOK(m)
+    && klonCanKV(this, k, v)
+
+    && CalidLineKV(k,v)
+  }
+
+
+
+
+
+
+
+  predicate {:isolate_assertions} CalidCanKey(k : Object)
+    //conditions an object to be added as a Key into the Klon map
+    //  note this doesn't seem to deal with ougoing field values, but that will get
+    //  caught eventually via  HeapContextReady() &  ValueContextReady()
+    //doesn't seem to require Calid????
+    //isn't this more eor less ownersInKlown>?>
+    //izn't thgs being replaced ie. tis dead
+    requires k.Ready() //&& k.Valid() // should context go in here too? probasbly?
+    //requires ownersInKlown(k) ///hmm, req or jsut in body?  Just In BODY!!! 31 Aug 2025
+
+    //pretty sure I want thewe two here to match CalidCanValue
+    requires o.Ready() //&& o.Valid()
+//    requires objectInKlown(o)  //THAT is clearly FUCKEDy
+
+    reads {}
+  {
+    && (k in oHeap)
+    && (k !in m.Keys)
+    && ownersInKlown(k)
+  }
+
+
+  predicate {:isolate_assertions} CalidCanValue(k : Object, v : Object)
+    //conditions an object to be added as a Value into the Klon map
+    // dunno if I really need this but wrote it anyway as an extenion of CanCalidKey above
+    //  note this doesn't seem to deal with ougoing field values, but that will get
+    //  caught eventually via  HeapContextReady() &  ValueContextReady()
+    //doesn't seem to require Calid????
+    requires k.Ready() //&& k.Valid() // should context go in here too? probasbly?
+    requires v.Ready() //&& v.Valid()
+    requires ownersInKlown(k)
+    requires o.Ready() //&& o.Valid()
+    requires objectInKlown(o)
+
+    requires CalidCanKey(k)
+
+    //the six requirements of preCalid2 / computeOwnerForClone apocalypse
+    requires k.owner <= m.Keys <= oHeap
+    requires m.Values <= hns()
+    requires o.Ready()
+    requires objectInKlown(o)
+    requires HeapOwnersReady()
+    requires c_amfx <= oHeap
+
+    reads oHeap, m.Values
+  {
+    && (v !in m.Values)
+    && (v.Ready()) //&& v.Valid() && v.Context(hns({v})))
+    && (CalidLineKV(k,v)) //will this do?
+  }
+
+
+
+  ghost predicate {:isolate_assertions} calidCanKV(k : Object, v : Object)
+    requires k.Ready() //&& k.Valid() // should context go in here too? probasbly?
+    requires v.Ready() //&& v.Valid()
+    requires ownersInKlown(k)
+    requires o.Ready() //&& o.Valid()
+    requires objectInKlown(o)
+
+
+    reads oHeap, m.Values
+
+  {
+    && SuperCalidFragilistic()
+    // && HeapContextReady()
+    // && ValuesContextReady()
+    // && Calid()
+    && CalidCanKey(k)
+    && CalidCanValue(k,v)
+  }
+
+
+
+
+  //[[[[[[[[[[[[[[[[[[[[[[[[[[[[[[[[[[[[[[[[]]]]]]]]]]]]]]]]]]]]]]]]]]]]]]]]]]]]]]]]
+  //[[[[[[[[[[[[[[[[[[[[[[[[[[[[[[[[[[[[[[[[]]]]]]]]]]]]]]]]]]]]]]]]]]]]]]]]]]]]]]]]
+
+
+
+
+  lemma {:isolate_assertions} CalidLineKVReflexive(k : Object, v : Object)
+    //speciefic
+    requires not(inside(k,o))
+    requires k == v
+
+    //generic?
+    requires k.Ready()
+    requires ownersInKlown(k)
+    requires v.Ready()
+    requires o.Ready()
+    requires objectInKlown(o)
+
+    //the six requirements of preCalid2 / computeOwnerForClone apocalypse
+    requires apoCalidse()
+
+    requires k in oHeap
+    requires forall x <- m.Keys :: outside(x,o) ==> (m[x] == x)
+//    requires forall x <- k.AMFO :: (m[o] == o)
+
+    ensures  checkOwnershipOfClone(k, v, this)
+    ensures  checkBoundOfClone(k, v, this)
+    ensures  mappingOwnersThruKlownKV(k,v,this)
+    ensures  CalidLineKV(k, v)
+  {
+
+    assert forall x <- m.Keys :: outside(x,o) ==> (m[x] == x);
+
+    assert not(inside(k,o));
+    assert k == v;
+    assert k != o;
+    assert k.AMFO == v.AMFO;
+    assert checkOwnershipOfClone(k, v, this);
+    assert k.owner == v.owner;
+    assert k.bound == v.bound;
+
+    k.ExtraReady();
+
+    assert m.Keys >= k.AMFX >= k.AMFB >= k.bound;
+    assert m.Keys >= k.AMFX >= k.owner;
+
+    assert outside(k,o);
+    //    ExternalOwnersAreOutside(k,o);
+    assert forall oo <- k.AMFX  :: outside(oo, o);
+    assert forall  x <- m.Keys  :: outside(x, o) ==> (m[x] == x);
+    assert forall oo <- k.AMFX  :: m[oo] == oo;
+    assert forall oo <- k.owner :: m[oo] == oo;
+
+    assert forall oo <- k.AMFB  :: outside(oo, o);
+    assert forall  x <- m.Keys  :: outside(x, o) ==> (m[x] == x);
+    assert forall oo <- k.AMFB  :: m[oo] == oo;
+    assert forall oo <- k.bound :: m[oo] == oo;
+
+assert v == k;
+assert v.bound == k.bound;
+
+    // assert (v.bound == mapThruKlon(k.bound, this));
+    // assert (v.owner == mapThruKlon(k.owner, this));
+
+    assert mappingOwnersThruKlownKV(k,v,this);
+
+  }
+
+  //[[[[[[[[[[[[[[[[[[[[[[[[[[[[[[[[[[[[[[[[]]]]]]]]]]]]]]]]]]]]]]]]]]]]]]]]]]]]]]]]
+  //[[[[[[[[[[[[[[[[[[[[[[[[[[[[[[[[[[[[[[[[]]]]]]]]]]]]]]]]]]]]]]]]]]]]]]]]]]]]]]]]
+
+///OwnersLine version
+
+
+//Need to WORK The FUCK out wwhat to do about THIS
+  ghost predicate {:isolate_assertions}   preOwners() : (r : bool)
+    reads oHeap, m.Values
+  {
+    // && HeapOwnersReady()    ///hmm
+    // && ValuesOwnersReady()
+    && (o.Ready() && (o in oHeap))
+    && (objectInKlown(o))  //KJXFUCK  do i want this in here? really?   ///Can U do without it??
+    && (o.AMFX == o_amfx)
+    && (flatten(clbound) >= o.AMFB)
+    && (o.AMFO == o_amfx+{o})
+    && (c_amfx >= flatten(clbound) >= flatten(o.bound))
+  }
+
+
+
+  ghost predicate {:isolate_assertions} preOwners2() : (r : bool)
+    reads {}
+  {
+    && (c_amfx <= oHeap) //should goto precalid1??
+    && ((o in m.Keys) ==> (
+        var c := m[o]; //WE HAS KLONE
+        && (c_amfx  == c.AMFX)
+        && (clowner == c.owner)
+        && (clbound == c.bound)
+       ))
+  }
+
+  ghost predicate {:isolate_assertions} SuperCalidOwners() : (r : bool)
+    reads oHeap, m.Values
+  {
+    // && HeapOwnersReady()
+    // && ValuesOwnersReady()
+    && CalidOwners()
+  }
+
+  ghost predicate {:isolate_assertions} CalidOwners() : (r : bool)
+    // requires  HeapOwnersReady()
+    // requires  ValuesOwnersReady()
+    reads oHeap, m.Values
+  {
+        // && HeapOwnersReady()
+        // && ValuesOwnersReady()
+    && apoCalidse()
+    && preOwners()
+    && preOwners2()
+    && (m.Keys <= oHeap)
+    && objectInKlown(o)
+    && (forall k <- m.Keys :: OwnersLineKV(k, m[k]))
+  }
+
+//does this mean it MUST be in or it CAN be in
+//with objectInKnown(k) this says it MUST ne in,. doesn;t it?
+//FUCK FUCK FUCK compare CalidLineKV!!!
+//ditto (v in hns({v}))) from earlier plain (v in hns())
+ predicate {:isolate_assertions} OwnersLineKV(k : Object, v : Object)
+    requires apoCalidse()
+    reads oHeap, m.Values
+  {
+//  && (k.Ready() && (objectInKlown(k)) && k in oHeap)   28 Oct 2025
+    && (k.Ready() && (ownersInKlown(k)) && k in oHeap)
+    && (v.Ready() && (v in hns({v})))
+
+ //   && (v.AMFO  >= v.AMFB  >= k.AMFB)  //GREENLAND
+    && (   (inside(k,o)) ==> (k.AMFB  <= o.AMFB))  //GREENLAND
+
+    && (not(inside(k,o)) ==> (v == k))
+    && (   (inside(k,o)) ==> ((v !in oHeap)) )
+
+  //MAPPING - KJXFEARSATAN
+    && (mappingOwnersThruKlownKV(k,v,this))
+  }
+
+
+//FROM DAHLIA
+
+lemma {:isolate_assertions} directOwnerInKlownIsEnough(o : Object)
+  requires o.Ready()
+  requires SuperCalidFragilistic()
+  requires o.owner <= m.Keys //note just direct owner
+   ensures ownersInKlown(o)
+{
+  assert forall x <- m.Keys :: objectInKlown(x);
+  assert flatten(o.owner) == o.AMFX <= m.Keys;
+  assert forall oo <- o.owner :: o.AMFX <= m.Keys;
+  assert ownersInKlown(o);
+}
+
+
+
+
+  lemma {:isolate_assertions}  FieldFromHeapContext(o : Object, n : string, v : Object)
+    //assert a bunch of stuff about a field - could become a function later
+    requires HeapContextReady()
+    requires o in oHeap
+    requires n in o.fields.Keys
+    requires v == o.fields[n]
+
+    ensures  v in o.fields.Values
+    ensures  v.Ready()
+    ensures  v.Valid()
+    ensures  v.Context(oHeap)
+    ensures  v in oHeap
+  {
+    assert o.Ready();
+    assert o.Valid();
+    FieldInFields(o,n,v);
+    assert v in o.fields.Values;
+    assert o.Context(oHeap);
+    assert o.fields.Values <= oHeap;
+    assert v in oHeap;
+    assert HeapContextReady();
+    assert forall x <- oHeap :: (x.Ready() && x.Valid() && x.Context(oHeap));
+    assert v.Ready() && v.Valid() && v.Context(oHeap);
+  }
+
+
+
+}//end datatype Klon
+///////////////////////////////////////////////////////////////////////////////////////////
+/////////////////////////////////////////////////////////////////////////////////////////
+///////////////////////////////////////////////////////////////////////////////////////////
+/////////////////////////////////////////////////////////////////////////////////////////
+///////////////////////////////////////////////////////////////////////////////////////////
+/////////////////////////////////////////////////////////////////////////////////////////
+///////////////////////////////////////////////////////////////////////////////////////////
+/////////////////////////////////////////////////////////////////////////////////////////
+///////////////////////////////////////////////////////////////////////////////////////////
+/////////////////////////////////////////////////////////////////////////////////////////
+///////////////////////////////////////////////////////////////////////////////////////////
+/////////////////////////////////////////////////////////////////////////////////////////
+
+///Important Klon Mappinhgs
+
+
+
+
+
+predicate {:isolate_assertions}  checkOwnershipOfClone(k : Object, v : Object, m : Klon)
+  //to work, this needs m.o and m.m[m.o] to be set up
+  //but does NOT need k in Keys, or v in values!
+  //
+  // apparently doesn't even need Caliud or precalid let alone supercalid.  HMMM
+  requires k.Ready()
+  requires m.ownersInKlown(k)
+  requires v.Ready()
+  requires m.apoCalidse()
+
+  //the six requirements of preCalid2 / computeOwnerForClone apocalypse
+  requires k.owner <= m.m.Keys <= m.oHeap
+  requires m.m.Values <= flatten( m.hns() )
+  requires m.o.Ready()
+  ///requires m.objectInKlown(m.o) //// NO NO NO NO NO NO NO NO NO
+  requires m.HeapOwnersReady()
+  requires m.c_amfx <= m.oHeap
+
+  reads m.oHeap, m.m.Values
+{
+  mappingOwnersThruKlownKV(k,v,m)
+}
+
+
+
+
+  predicate {:isolate_assertions} mappingOwnersThruKlownKV(k : Object, v : Object, m : Klon) : (r : bool)
+    //KJX FEAR SATAN
+    //this vrsion currently matches CalidLineKV, i.e. k and v don't have to be in the klon
+    //but that means we can't mapp intl and AMFO  //um,,
+    //i think this is th4e INVARIANT
+    //Sure seeems to be the  INVARIANT -- 22 Dec 2025
+
+   decreases k.AMFO
+    requires m.apoCalidse()
+    requires m.ownersReadyInKlown(k)
+//    requires v.Ready()
+    reads m.oHeap, m.m.Values
+    {
+      // KJX FEAR SATAN!!
+
+      if (k == m.o) then (
+          && (v == m.m[m.o])
+          && (v.owner == m.clowner)
+          && (v.bound == m.clbound)
+        ) else if (outside(k, m.o) )
+          then (
+            k == v
+        ) else (
+          assert strictlyInside(k, m.o);
+              // && (v.bound == mapThruKlon(k.bound, m))
+              // && (v.owner == mapThruKlon(k.owner, m))
+              && mappingOWNRsThruKlownKV(k.bound, v.bound, m)
+              && mappingOWNRsThruKlownKV(k.owner, v.owner, m)
+        )
+    }
+
+
+
+    //our shold this be MAPPING Owners?????
+    //note that this is called ONLY strictly wihin the pivot - see the JDVANCE note
+    predicate {:isolate_assertions} mappingOWNRsThruKlownKV(kk : OWNR, vv : OWNR, m : Klon) : (r : bool)
+      //actual OWNR version of mappingOwnersThruKlownKV
+      //within the pivot anyway!
+      //KJX FEAR SATAN
+          //OK so wher doe this asy "inside the pivot"?   - it DO#ESNT
+          //does that matter?  who knows?
+      requires m.apoCalidse()
+      // requires AllReady(kk)  // 29 Oct 2025
+      // requires AllReady(vv)  // 29 Oct 2025
+      requires kk <= m.m.Keys
+  ////requires vv <= m.m.Values  ///hmm must be trie if kjk,s inside Klon...
+  ////requires kk > m.o.AMFO  //gotta be inside kloned bit..  //JDVANCE yeah shoud do that!
+
+        {
+//I have NO FUCKING IDEA if this is dong te RIGHT THING or not.
+//anin't that great.
+//i think its dong CLOSE ENOUGH to the right thing for a paper
+//the visualisations all look OK now
+//but stil - 21 Sept 2025
+
+
+        && (vv == (mapThruKlon(kk - m.o.AMFO, m) + m.m[m.o].AMFO))
+        && (flatten(kk) <= m.oHeap)
+        && (flatten(vv) <= m.hns(vv))
+
+          // var inside1 := kk - m.o.AMFO;
+          // var option1 := mapThruKlon(inside1,m) + m.m[m.o].AMFO;
+          // (vv == option1)
+        }
+
+
+
+function {:isolate_assertions} computeOwnerForClone(oo : Owner, m : Klon) : (nuowner : Owner)
+  //given some flattened Owner oo, calculate the mapped / cloned version
+  //EXCEPT OWNERS SHOULDNT BE FLATTENNED!!!
+///TODO//Libertarian  //requires (flatten(oo) >= m.o.AMFO)   //should this be there or not?
+  //
+  //     7 Aug 2025 - kjx thinks - this doesn't work if we're flatting the bound
+  //             I removed the constraint hopijng it doesn't break too  much stuff..
+  //
+  //  I think this makes sense for owners of subparts being clonedj
+///  but not neccessarily for e..g bounds that lie (partially) outside?
+///
+  //  Ha! remember that in many (if not all) cases. bound == owner
+  //    which means that, it pretty much needs to have the same mapping...
+  //
+///seemss to survive without oo being ready!
+///seemss to survive without ANYUTHING being Ready
+///KJXA Naa will need Values...
+  requires m.apoCalidse()  //note that this requires m.o already in m.m.Keys
+  requires oo <= m.m.Keys
+//  requires flatten(oo) >= m.o.AMFO //hmmmA
+  requires m.SuperCalidFragilistic()
+   ensures nuowner <= m.hns()
+   ensures flatten(oo) <= m.oHeap //so this MUST be preexisting.
+   ensures flatten(nuowner) <= m.hns()
+   ensures mappingOWNRsThruKlownKV(oo, nuowner, m)   //rather important
+       //yes 'rathr imoportant" infdeed,
+
+
+   ensures nuowner == global(sideways(local(oo, m),m),m)
+ //   ensures nuowner == shiftAMFOZ(oo, m.o.AMFO,  m.m[m.o].AMFO, m.m)
+
+      //********also important that that's OWNRES NOT Owners **************//
+      //***ot is it??
+      //JDVANCE -- note that sholdlj constraint oo to be inside(the pivot)
+      //so the new owner is strictly inside the blivet..../
+ // requires flatten(oo) >= m.o.AMFO           //JDVANCE
+
+ reads m.oHeap, m.m.Values
+//  reads {}
+{
+  assert m.ValuesContextReady();
+  var inside1 := oo - m.o.AMFO;
+  assert inside1 <= m.oHeap;
+
+  var nuowner := mapThruKlon(inside1,m) + m.m[m.o].AMFO;
+
+  assert nuowner == (set x <- (oo - m.o.AMFO) :: m.m[x]) + m.m[m.o].AMFO;
+//  assert nuowner == shiftAMFOZ(oo, m.o.AMFO,  m.m[m.o].AMFO, m.m);
+
+  assert mapThruKlon(inside1,m) <= m.m.Values <= m.hns();
+  assert m.m[m.o] in m.hns();
+  assert m.ValueInContext(m.m[m.o]);
+  assert m.m[m.o].AMFO <=  m.hns();
+
+  var fuck1 := local(oo, m);
+  var fuck2 := sideways(fuck1, m);
+  var fuck3 := global(fuck2, m);
+  assert fuck3 == nuowner;
+
+  assert fuck3 == global(sideways(local(oo, m),m),m);
+
+
+//  .AMFO <= m.m.Values <= m.hns();ƒƒ∂çƒ©
+  assert nuowner <= m.hns();
+  nuowner
+}
+//really this is to MATCH the checkClownershipINSIDE
+
+
+
+
+
+
+
+
+
+
+
+
+
+
+
+
+
+
+
+///////////////////////////////////////////////////////////////////////////////////////////
+/////////////////////////////////////////////////////////////////////////////////////////
+
+predicate klonVMapOK(m : vmap<Object,Object>, ks : set<Object> := m.Keys)
+  requires ks <= m.Keys
+  //klonVMapOK the vmap parts of a klon are OK
+  //still need to do something for iHeap and ns etc
+  //should probably swizzle this to take a Klon, not a vmap/...
+  //KJX AND that shoud something like klonReady
+  //meaning that for all targets (m.Keys)
+  //the coresponding klon  m[k] is
+  // - ready
+  // - corresponds to the target
+  //structure of this needs TO MATCH THE CALIDs and
+  //object invairants ready, valid, calid, etc
+  //klonca
+  // IDEALLY the "mapThru" features shouldn't be part of
+  // the invariuant itself (klonOK) NOR the extension test (klonCanKV)
+  // no the extension (klonKV)
+  // rather mapThru etc should be post-derivable efrom calid, not wired in...
+  //  which hopefully is ONE clause per "field" of Dahlia's "Object" and no more?
+  reads m.Values`fieldModes
+  reads ks`fieldModes
+{
+//Readiness???  //KJXFEARSATAN
+   && (forall k <- ks :: k.Ready() && m[k].Ready() )
+
+  //AMFO
+  && (forall k <- ks :: k.AMFO <= m.Keys)
+  //  && (forall k <- ks :: mapThruVMap(k.AMFO, m) == m[k].AMFO)
+
+  //AMFB
+  && (forall k <- ks :: k.AMFB <= m.Keys)
+  //  && (forall k <- ks :: mapThruVMap(k.AMFB, m) == m[k].AMFB)
+
+  //KJXOWNERS
+  //region & owners?
+  //  && (forall x <- ks :: x.owaner <= x.AMFO)//KJXOWNERS
+//  && (forall x <- ks :: x.bound <= x.owner <= m.Keys) //should that bound be ks?
+  //  && (forall k <- ks :: mapThruVMap(k.owner, m) == m[k].owner)
+  //  && (forall k <- ks :: mapThruVMap(k.bound, m) == m[k].bound)
+
+  //field values? //KJX
+  //
+  //
+  //  && (forall k <- ks :: k.fieldModes == m[k].fieldModes)
+///
+  //see rant above
+}
+
+
+
+  function {:isolate_assertions} {:timeLimit 60} klonKV(m' : Klon, k : Object, v : Object) : (m : Klon)   //TIME-3-OCT
+    //aux function for adding k v to a m' giving m
+//Klon.CalidKV does all the real work!
+  requires k !in m'.m.Keys
+  requires v !in m'.m.Values
+  requires klonVMapOK(m'.m)
+  requires klonCanKV(m', k, v)
+
+  ensures klonVMapOK(m.m)
+  ensures klonCanKV(m', k, v)
+//  ensures forall x <- m.m.Keys, y <- m.m.Values :: (y == v) ==> (x == k)
+  ensures m == m'.(m:=m'.m[k:=v])
+  ensures m.from(m')
+  ensures m.m.Keys   == m'.m.Keys+{k}
+  ensures m.m.Values == m'.m.Values+{v}
+  ensures m.o        == m'.o
+  ensures m.oHeap    == m'.oHeap
+  ensures forall z <- m'.m.Keys :: modesEQ(m'.m[z].fieldModes, m.m[z].fieldModes)
+
+  reads k, v, m'.oHeap, m'.hns(), m'.m.Keys, m'.m.Values
+
+  //   reads k`fields, k`fieldModes
+  //   reads v`fields, v`fieldModes
+  //
+  //   reads m'.oHeap`fields, m'.oHeap`fieldModes
+  //   reads m'.ns()`fields,  m'.ns()`fieldModes
+    reads m'.m.Keys`fields, m'.m.Keys`fieldModes
+    reads m'.m.Values`fields, m'.m.Values`fieldModes
+
+  //reads  m'.m.Values, m'.oHeap  //for ValuesContextReady?
+{
+  assert klonVMapOK(m'.m);
+  assert klonCanKV(m', k, v);
+  assert forall x <- m'.m.Keys, y <- m'.m.Values :: (y == v) ==> (x == k);
+    // var m'fmodes := map z <- m'.m.Keys :: z := z.fieldModes;
+    // assert m'fmodes.Keys == m'.m.Keys;
+    // assert forall z <- m'.m.Keys :: modesEQ(z.fieldModes, m'fmodes[z]);
+
+  var r0 : vmap<Object,Object> := vmapKV(m'.m,k,v); // m'.m[k:=v];
+  assert klonVMapOK(r0);
+  assert r0 ==  m'.m[k:=v];
+// assert forall z <- m'.m.Keys :: modesEQ(z.fieldModes, m'fmodes[z]);
+// assert forall z <- m'.m.Keys :: modesEQ(r0[z].fieldModes, m'fmodes[z]);
+
+  var r1 := m'.(m:=r0);
+  assert r1 == m'.(m:=m'.m[k:=v]);
+
+  haventFuckedFieldModes(m',k,v,r1);
+
+//  assert forall z <- m'.m.Keys :: z.fieldModes == r1.m[z].fieldModes;
+  r1
+  }
+
+//
+// //[[[[[[[[[[[[[[[[[[[[[[[[[[[[[[[[[[[[[[[[]]]]]]]]]]]]]]]]]]]]]]]]]]]]]]]]]]]]]]]]
+//
+
+predicate modesEQ(a : map<string,Mode>, b : map<string,Mode>)
+ { (a.Keys == b.Keys) && (forall n <- a.Keys :: a[n] == b[n]) }
+
+
+  lemma {:isolate_assertions} {:timeLimit 30} haventFuckedFieldModes(m' : Klon, k : Object, v : Object, m : Klon)
+    requires k !in m'.m.Keys
+    requires v !in m'.m.Values
+    requires klonVMapOK(m'.m)
+    requires klonCanKV(m', k, v)
+    requires m == m'.(m:=m'.m[k:=v])
+     ensures forall z <- m'.m.Keys :: modesEQ(m'.m[z].fieldModes, m.m[z].fieldModes)
+{
+    var m'fmodes := map z <- m'.m.Keys :: z := m'.m[z].fieldModes;
+    assert m'fmodes.Keys == m'.m.Keys;
+    assert forall z <- m'.m.Keys :: modesEQ(m'.m[z].fieldModes, m'fmodes[z]);
+    assert forall z <- m'.m.Keys :: modesEQ(m. m[z].fieldModes, m'fmodes[z]);
+    assert forall z <- m'.m.Keys :: modesEQ(m'.m[z].fieldModes, m.m[z].fieldModes);
+}
+
+//
+//
+//
+// //[[[[[[[[[[[[[[[[[[[[[[[[[[[[[[[[[[[[[[[[]]]]]]]]]]]]]]]]]]]]]]]]]]]]]]]]]]]]]]]]
+//
+
+predicate klonCanKV(m' : Klon, k : Object, v : Object)
+  //extending m' with k:=v will be klonVMapOK
+  // requires klonVMapOK(m'.m)  //should this be here?  if not, in below!  //BOWIE
+
+  //requires m'.HeapContextReady()     //wuld be nice but fucks callers' read clauses?
+  //requires m'.ValuesContextReady()
+  //requires Calid() ?????
+
+///does not check ownerhsip!!!
+
+  reads k, v, m'.oHeap, m'.hns(), m'.m.Keys, m'.m.Values
+  // reads k`fields, k`fieldModes
+  // reads v`fields, v`fieldModes
+  //
+  // reads m'.oHeap`fields, m'.oHeap`fieldModes
+  // reads m'.ns()`fields,  m'.ns()`fieldModes
+  // reads m'.m.Keys`fields, m'.m.Keys`fieldModes
+  // reads m'.m.Values`fields, m'.m.Values`fieldModes
+{
+  && klonVMapOK(m'.m) //BOWIE
+  && canVMapKV(m'.m, k, v)
+  && (k in m'.oHeap)  //KJX do I want this here?
+  && (if (v==k) then (v in m'.oHeap) else (v !in m'.oHeap)) //nope - happens after  wards
+
+  //grrr. should refactor this
+  && k.Ready() && k.Valid() && k.Context(m'.oHeap)
+  && v.Ready() && v.Valid() && v.Context(m'.hns({v}))
+
+  //  && k.Context(m'.m.Keys+{k})  ///what IS this?
+  &&  m'.ownersInKlown(k)
+  && (k.fieldModes == v.fieldModes)//hhhmm see anbove
+
+  //  && (v.AMFX >= v.AMFB >= k.AMFB) //is this right?   really?
+  //17 June 2025 kjx thinks this iswrong & shoud be in CalidLineKV
+
+
+  //END DOOUBLE BOWIE
+}
+
+// basic mappings
+
+
+function {:isolate_assertions} mapThruKlon(os: set<Object>, m : Klon) : (r : set<Object>)
+  //image of os under klon mapping m
+  // reads m.m.Keys`fields, m.m.Keys`fieldModes
+  // reads m.m.Values`fields, m.m.Values`fieldModes
+  requires os <= m.m.Keys
+   ensures r  <= m.m.Values
+   ensures (os > {}) ==> (r > {})
+  reads {}
+    { assert (os > {}) ==> ( var x :| x in os; {m.m[x]} > {});  //THIS LINE IS OF SATAN. WASBN"T NEEDED PREVIOUSLY.,..
+      set o <- os :: m.m[o] }
+
+function mapBackKlon(os: set<Object>, m : Klon) : (r : set<Object>)
+  //image of os under INVERSE klon mapping m
+  // reads m.m.Keys`fields, m.m.Keys`fieldModes
+  // reads m.m.Values`fields, m.m.Values`fieldModes
+  requires os <= m.m.Values
+  ensures  r  <= m.m.Keys
+  reads {}
+{ mapBackVMap(os,m.m) }
+
+
+
+
+
+
+predicate {:isolate_assertions} istKlonnyKlon(os : Owner, ks : set<Object>, m : Klon)
+    requires m.o.Ready()
+    requires m.objectInKlown(m.o)
+    requires os <=  m.m.Keys <= m.oHeap
+    requires m.c_amfx <= m.oHeap
+    requires m.apoCalidse()
+    requires m.SuperCalidFragilistic()
+
+     reads m.oHeap, m.m.Values
+
+    decreases os, 50
+{
+  && (forall o <- os :: o in m.m.Keys)
+  && (m.o in os)
+  && (computeOwnerForClone(os, m) == ks)  ///AMOST CERTAINLY WRONG!!!!!  --- should call checkOwnershipOfClone instead
+}
+
+predicate istKlonAlleFelder(o : Object, k : Object, m : Klon)
+  reads o`fields, o`fieldModes
+  reads k`fields, k`fieldModes
+{
+  && (o.fields.Keys     == k.fields.Keys)
+  && (o.fieldModes.Keys == k.fieldModes.Keys)
+  && (o.fields.Values     <= m.m.Keys)
+  && (forall f <- o.fields.Keys :: (m.m[o.fields[f]]  == k.fields[f]))
+//  && ()   //at some point needs to check mapping for fieldModes?    //OR NOT///
+}
+
+
+///// special purpose mappings - local/globa/sideways
+
+function local(o : OWNR, m : Klon) : (r : OWNR)
+ //take a "global" original OWNR to a local internal one in the original (should this be global2local)
+ //should theyb e differen types? ARGH!
+  // //requires isFlat(o)
+  // //ARGH.  this is a set of Owners inside the pivotg
+  // //but those objects are all fully global AMDOs...?
+  // requires m.apoCalidse()
+  // requires o >= m.o.AMFO   //o >= or o > ?
+   ensures r <= o
+   //ensures isFlat(r)
+   // { o - m.o.AMFO  }   //shit shit shit
+   { o - m.o.AMFO  }
+
+function {:isolate_assertions} global(oo : set<Object>, m : Klon) : (rs : set<Object>)
+ //take a "local" OWNR to a global one in the clone (should this be local2global)
+   requires m.apoCalidse()
+  //  requires forall o <- oo :: inside(o,m.m[m.o])
+  //  //ensures  isReallyFuckingFlat(rs)
+  // //requires o >= m.o.AMFO
+  //  //ensures isFlat(r)
+   { oo + m.m[m.o].AMFO  }
+
+function sideways(oo : set<Object>, m : Klon) : (r : set<Object>)
+ //take a "local" OWNR to a global one in the clone (should this be local2global)
+  //  requires AllReady(oo)
+   requires oo <= m.m.Keys
+  //  requires m.apoCalidse()
+  // //requires isFlat(o)
+  // requires oo <= m.o.AMFO
+  //  //ensures isFlat(r)
+  ensures r ==  mapThruKlon(oo, m) //hmm???
+  ensures r <= m.m.Values
+   { mapThruKlon(oo, m) }
+
+
+
+
+
+
+
+
+
+
+
+
+
+
+predicate checkBoundOfClone(k : Object, v : Object, m : Klon) { nuBoundsOK(k.owner, k.bound) }
