Printing.dfy
@@ -1,0 +1,915 @@
+include "Klon.dfy"
+include "Library.dfy"
+include "Set-Lemmata.dfy"
+
+
+method printobject(o : Object)
+{
+      printobj(o);
+      print "\n  owner:";
+      printset(o.owner);
+      print "\n   AMFO:";
+      printset(o.AMFO);
+      print "\n   AMFB:";
+      printset(o.AMFB);
+      print "\n";
+      printobjfields(o);
+}
+
+method printset(s : set<Object>)
+{
+  var t := s;
+  while t != {}
+    decreases t
+  {
+    var y: Object;
+    y :| y in t;
+    printobj(y);
+    print " ";
+    t := t - {y};
+  }
+}
+
+
+method printobjectset(s : set<Object>)
+{
+  var t := s;
+  while t != {}
+    decreases t
+  {
+    var y: Object;
+    y :| y in t;
+    printobject(y);
+    print "- - - - - - - -\n";
+    t := t - {y};
+  }
+}
+
+
+function fmtobj(o : Object) : string
+   reads o
+{
+  "Obj(" + o.nick + ")"
+}
+
+method printobj(o : Object)
+  ensures unchanged(o)
+  modifies {}
+{
+ print "Obj(", o.nick, ")";
+}
+
+
+function fmtown(oo : Owner) : string
+   reads oo
+{
+  "Own(" + fmtnickset(oo) + ")"
+}
+
+method printown(oo : Owner)
+  ensures unchanged(oo)
+  modifies {}
+{
+ print fmtown(oo);
+}
+
+
+//should alos print field modes?
+method printobjfields(o : Object)
+{
+  var t := o.fields;
+  while t != map[]
+    decreases t
+  {
+    var y: string;
+    y :| y in t.Keys;
+    print " ";
+    print y,":=";
+    printobj(t[y]);
+    print " ",
+      if (refOK(o,t[y])) then "refOK" else "***NOT REFOK***";
+    t := t - {y};
+    print "\n";
+  }
+}
+
+
+method {:isolate_assertions} printklon(m :  Klon)
+  modifies {}
+
+  requires m.HeapContextReady()
+  requires m.ValuesContextReady()
+  ensures unchanged(m.oHeap,m.hns())
+  ensures unchanged(m.m.Keys,m.m.Values, m.o)
+  ensures forall k <- m.m.Keys   :: unchanged(k)
+  ensures forall v <- m.m.Values :: unchanged(v)
+  ensures old(m.Calid()) == m.Calid()
+  {
+    printmapping(m.m);
+  }
+
+method printmapping(m : vmap<Object,Object>)
+  modifies {}
+  ensures unchanged(m.Keys,m.Values)
+  ensures forall k <- m.Keys   :: unchanged(k)
+  ensures forall v <- m.Values :: unchanged(v)
+{
+  var t := m;
+  while t != map[]
+    decreases t
+  {
+    var y: Object;
+    y :| y in t.Keys;
+    print " ";
+    printobj(y);
+    print ":=";
+    printobj(t[y]);
+    t := t - {y};
+    print "\n";
+  }
+}
+
+
+
+method printmappingIsIsomorphic(m: vmap<Object,Object>, o : Object, os : set<Object>)
+{
+  var t := m;
+  while t != map[]
+    decreases t
+  {
+    var y: Object;
+    y :| y in t.Keys;
+    print " ";
+    printobj(y);
+    print ":=";
+    printobj(t[y]);
+    print "  ";
+//    print isIsomorphicMappingOWNED(y, o, m, os);
+    print "\n";
+    t := t - {y};
+   }
+}
+
+
+method jeSuisClone(src : Object, m : Klon, context : set<Object>) returns (rv : bool)
+  requires src in m.m.Keys
+  requires src in context
+  requires m.m.Keys   <= context
+  requires m.m.Values <= context
+{ return false; }
+
+
+//iterative clone-checker, most likely only dynamic at this point
+method  istEinKlon(src : Object, m : Klon, context : set<Object>) returns (rv : bool)
+ //probably needs CallOK(context)  for a start!
+    requires m.o.Ready()
+    requires m.objectInKlown(m.o)
+    requires src.Ready()
+    requires m.objectInKlown(src)
+
+  requires m.SuperCalidFragilistic()
+
+  requires src in m.m.Keys
+  requires src in context
+  requires m.m.Keys   <= context
+  requires m.m.Values <= context
+{
+  rv := true;
+  var os := context;
+  while os != {}
+    decreases os
+    invariant os <= context
+  {
+    var o: Object;
+    o :| o in os;
+    os := os - {o};
+
+    if (outside(o,src)) { print "   skipping "+fmtobj(o)+" outside src\n"; continue; }
+    if (o !in m.m.Keys) { print "   skipping "+fmtobj(o)+" outside Klon \n"; continue; }
+
+    var k := m.m[o];  //k klon of o
+
+    print "   checking ",fmtobj(o)," cloned as ",fmtobj(k), " ";
+
+    assert (o.bound <= m.m.Keys) by  {assert m.objectInKlown(o);}
+    assert (o.owner <= m.m.Keys) by  {assert m.objectInKlown(o);}
+
+    rv :=
+         && istKlonnyKlon(o.bound, k.bound, m)
+         && istKlonnyKlon(o.owner, k.owner, m)
+         && istKlonAlleFelder(o, k, m)
+         ;
+
+   print rv,"\n";
+  }
+}
+
+
+
+function fmtnickset(Y: set<Object>) : string
+ reads Y`nick
+ {
+   fmtsetstr( set y <- Y :: y.nick )
+ }
+
+method mlurk(x: set<string>) returns (r: string)
+ requires |x| > 0
+ {
+  r :| r in x;
+ }
+
+
+lemma {:axiom} StrLEQ1(a : string,  b : string)
+  ensures (strLEQ(a, b) && strLEQ(b, a)) <==> (a == b)
+
+lemma {:axiom}  StrLEQ2(a : string,  b : string, c : string)
+  ensures (strLEQ(a, b) && strLEQ(b, c)) ==> strLEQ(a, c)
+
+lemma {:axiom} StrLEQ3(a : string,  b : string)
+  ensures  strLEQ(a, b) || strLEQ(b, a)
+
+lemma {:axiom} StrLEQ4(a : string)
+  ensures  strLEQ(a, a)
+{}
+
+
+ghost function anyOneOf(s: set<string>) : string
+  requires |s| > 0
+{
+  ExtractFromNonEmptySet(s)
+ }
+
+
+predicate IAMTheRessurection(s: set<string>, m : string)
+{
+  m in s && forall x <- s :: strLEQ(m, x)
+}
+
+predicate OnlyRessurection(s: set<string>, m : string)
+  requires m in s
+  requires IAMTheRessurection(s,m)
+  {
+   forall x <- s | IAMTheRessurection(s,x) :: x == m
+  }
+
+lemma ReallyJustOneRessurection(s: set<string>,  m : string, mm : set<string>)
+  requires m in s
+  requires IAMTheRessurection(s,m)
+  requires mm == set x <- s | IAMTheRessurection(s,x) :: x
+  //ensures |mm| == 1
+  ensures mm == {m}
+  {
+    OneRessurection(s,m);
+  }
+
+lemma OneRessurection(s: set<string>, m : string)
+  requires m in s
+  requires IAMTheRessurection(s,m)
+  ensures  forall x <- s | IAMTheRessurection(s,x) :: x == m
+{
+  assert m in s;
+  forall x <- s | IAMTheRessurection(s,x)
+    ensures  x == m //by
+      {
+         if (x == m) {
+           assert IAMTheRessurection(s,m);
+           assert strLEQ(x,m);
+           assert strLEQ(m,x);
+           assert IAMTheRessurection(s,x);
+           assert x == m;
+         } else {
+            assert {:contradiction} IAMTheRessurection(s,m);
+            assert {:contradiction} x in s;
+            assert {:contradiction} strLEQ(m,x);
+            assert {:contradiction} IAMTheRessurection(s,x);
+            assert {:contradiction} m in s;
+            assert {:contradiction} strLEQ(x,m);
+            StrLEQLEQIsEQ(x,m);
+            assert {:contradiction} x == m;
+            assert {:contradiction} false;
+         }
+      }
+}
+
+lemma LemmaSTREQ(x : string, y : string)
+ ensures (x == y) ==> strLEQ(x,y)
+ ensures (x == y) ==> strLEQ(y,x)
+{}
+
+lemma MemmaSTREQ(s : set<string>)
+    requires |s| == 1
+  ensures exists m <- s :: m in s
+  ensures exists m <- s :: forall x <- s :: strLEQ(m, x)
+   {
+     //var v : string :| v in s;
+     var v := ExtractFromSingleton(s);
+     assert s == {v};
+     forall x <- s ensures x == v  {
+      if (x == v) {
+          LemmaSTREQ(x,v);
+          assert strLEQ(x,v) && strLEQ(v,x);
+          assert forall x <- {v} :: strLEQ(v, x);
+          assert forall x <- s :: strLEQ(v, x);
+          assert exists m <- s :: forall x <- s :: strLEQ(m, x);
+          return; }
+      assert x != v;
+      LemmaSingletonEquality(s, x, v);
+      assert {:contradition} x == v;
+      assert {:contradition} false;
+     }
+     assert forall x <- s :: x == v;
+
+    forall x <- s ensures strLEQ(x,v) {
+        assert x == v;
+        LemmaSTREQ(x,v);
+        assert  strLEQ(x,v);
+    }
+   }
+
+
+lemma MummaSTREQ(s : set<string>)
+//unfinished - wasted LOTS of time on this now
+    decreases s
+    requires |s| > 0
+    // ensures  exists m <- s :: m in s
+    // ensures  exists m <- s :: forall x <- s :: strLEQ(m, x)
+   {
+     if (|s| == 1) { MemmaSTREQ(s); return; }
+     assert |s| > 1;
+     var v : string :| v in s;
+     var t := s - {v};
+     MummaSTREQ(t);
+//     assert exists m <- t :: forall x <- s :: strLEQ(m, x);
+
+//     var q  : string :| q in s && forall x <- s :: strLEQ(q, x);
+
+
+
+   }
+
+
+
+
+lemma EveryPlanetHasANorth(s : set<string>)
+  requires |s| > 0
+  // ensures  exists m <- s :: forall x <- s :: strLEQ(m, x)
+  // ensures  forall m <- s, n <- s ::
+  //     (&& (forall x <- s :: strLEQ(m, x))
+  //      && (forall x <- s :: strLEQ(n, x))) ==> (m == n)
+{
+      assert forall x <- s :: x == x;
+      forall x <- s ensures (strLEQ(x,x)) //by
+        {
+         LemmaSTREQ(x,x);
+         assert strLEQ(x,x);
+        }
+      assert forall x <- s :: strLEQ(x,x);
+      assert forall x <- s :: exists y <- s :: x == y;
+      assert forall x <- s :: exists y <- s :: strLEQ(x,y);
+
+}
+
+
+lemma DAFNY_IS_SATAN(s: set<string>)
+  requires s > {}
+   ensures forall m <- s, n <- s |
+              (&& (forall x <- s :: strLEQ(m, x))
+               && (forall x <- s :: strLEQ(n, x))) :: m == n
+{
+  var min := SetStrMin(s);
+  assert min in s;
+  assert IAMTheRessurection(s,min);
+  OneRessurection(s,min);
+  assert forall x <- s | IAMTheRessurection(s,x) :: x == min;
+  assert forall m <- s, n <- s |
+              (&& IAMTheRessurection(s,m)
+               && IAMTheRessurection(s,n)) :: min == m == n;
+  assert forall m <- s, n <- s |
+              (&& (forall x <- s :: strLEQ(m, x))
+               && (forall x <- s :: strLEQ(n, x))) :: m == n;
+}
+
+function IAMTheLife(s: set<string>) : (m : string)
+  requires |s| > 0
+  requires exists m <- s :: forall x <- s :: strLEQ(m, x)
+  requires forall m <- s, n <- s |
+      (&& (forall x <- s :: strLEQ(m, x))
+       && (forall x <- s :: strLEQ(n, x))) :: m == n
+
+  ensures  forall x <- s :: strLEQ(m, x)
+  {
+    assert exists m <- s :: forall x <- s :: strLEQ(m, x);
+    var m :| (&& (m in s)
+              && (forall x <- s :: strLEQ(m,x))
+              && (forall m <- s, n <- s |
+                    (&& (forall x <- s :: strLEQ(m, x))
+                     && (forall x <- s :: strLEQ(n, x))) :: m == n)
+             );
+    m
+  }
+
+///      var m :| m in s && (forall x <- s :: strLEQ(m,x);
+
+// ghost function IAMTheLife(s: set<string>) : (m : string)
+//   requires |s| > 0
+//   ensures  IAMTheRessurection(s,m)
+//   {
+//    var mm :| mm in s && IAMTheRessurection(s,mm); mm
+//   }
+//
+//
+// lemma ThereIsOneTrueFaith(s: set<string>)
+//   requires |s| > 0
+//   ensures exists m <- s :: IAMTheRessurection(s, m)
+//   {
+//     if (|s| == 1)
+//        {
+//         var m := theOneAndOnly(s);
+//         assert strLEQ(m,m);
+//         assert forall x <- s :: x == m && strLEQ(x,m);
+//         assert IAMTheRessurection(s, m);
+//         assert exists m <- s :: IAMTheRessurection(s, m);
+//        }
+//     else
+//     {
+//       assert |s| > 1;
+//       var guess :| guess in s;
+//       var rest  := s - {guess};
+//       assert s == ({guess} + rest);
+//       ThereIsOneTrueFaith(rest);
+//       var bestOfTHeRest := IAMTheLife(rest);
+//       assert IAMTheRessurection(rest, bestOfTHeRest);
+//       if (strLEQ(guess,bestOfTHeRest))
+//          {
+//           assert s == ({guess} + rest);
+//           assert IAMTheRessurection(s, guess);
+//           assert exists m <- s :: IAMTheRessurection(s, m);
+//          } else {
+//           assert s == ({guess} + rest);
+//           assert IAMTheRessurection(s, bestOfTHeRest);
+//           assert exists m <- s :: IAMTheRessurection(s, m);
+//          }
+//     assert exists m <- s :: IAMTheRessurection(s, m);
+//     }
+//  assert exists m <- s :: IAMTheRessurection(s, m);
+// }
+
+
+// function theOneAndOnly(s: set<string>) : (rv : string)
+//   requires |s| == 1
+//   ensures s == {rv}
+//   ensures IAMTheRessurection({rv}, rv)
+//   ensures IAMTheRessurection(s, rv)
+// {
+//   OneRessurection(s,rv);
+//   ExtractFromSingleton(s)
+// }
+
+
+ghost function thereIsOneThere(s: set<string>) : string
+  requires |s| > 0
+  ensures thereIsOneThere(s) in s
+{
+  var q :| q in s;
+  q
+}
+
+
+
+
+//probalby have to split the bloody thing tand use StrLEQIsTrans to deal with it...
+function fmtsetstr(Y: set<string>) : string
+ {
+  if (|Y| < 1) then ("") else (
+      assert |Y| >= 1;
+      assert exists y :: y in Y;
+
+  var s := Y;
+  assert |s| > 0;
+  SetStrHasMinimum(s);
+  DAFNY_IS_SATAN(s);
+  assert exists m <- s :: forall x <- s :: strLEQ(m, x);
+  assert forall m <- s, n <- s |
+      (&& (forall x <- s :: strLEQ(m, x))
+       && (forall x <- s :: strLEQ(n, x))) :: m == n;
+
+
+      var y := IAMTheLife(Y);
+      y +
+      (if (|Y| <= 1) then "" else " ")
+      + fmtsetstr( Y - {y} ) )
+  }
+
+
+lemma  {:isolate_assertions} SetStrHasMinimum(s : set<string>)
+  requires |s| > 0
+   ensures forall m <- s ::  m == m
+   ensures forall m <- s ::  strLEQ(m, m)
+   ensures exists m : string <- s :: forall x <- s ::  strLEQ(m, x)
+{
+   forall m <- s ensures strLEQ(m, m)  { StrEQISstrLEQ(m,m); }
+
+   var min :| min in s;
+   var done := {min};
+   var rest := s - done;
+   assert forall x <- done :: strLEQ(min, x);
+
+   while (rest > {})
+     decreases rest
+     invariant rest == (s - done)
+     invariant forall x <- done :: strLEQ(min, x)
+     invariant min in s
+     {
+      var next :| next in rest;
+      assert forall x <- done :: strLEQ(min, x);
+      if not(strLEQ(min, next)) {
+          StrNEQLEQ(min, next);
+          assert strLEQ(next, min);
+          forall x <- done ensures strLEQ( next, x)
+            { StrLEQIsTrans(next, min, x); }
+          min := next;
+          assert strLEQ(min, next);
+          assert forall x <- done :: strLEQ(min, x);
+          assert forall x <- done+{next} :: strLEQ(min, x);
+      }
+      done := done + {next};
+      rest := rest - {next};
+      assert rest == s - done;
+     }
+     assert forall x <- done :: strLEQ(min, x);
+     assert rest == {};
+     assert rest == s - done;
+     SetMinus0(s,done);
+     assert s <= done;
+}
+
+
+
+lemma  {:isolate_assertions} SetStrMin(s : set<string>) returns (min : string)
+  requires |s| > 0
+   ensures forall m <- s ::  m == m
+   ensures forall m <- s ::  strLEQ(m, m)
+   ensures exists m : string <- s :: forall x <- s ::  strLEQ(m, x)
+   ensures forall x <- s :: strLEQ(min, x)
+   ensures min in s
+{
+   forall m <- s ensures strLEQ(m, m)  { StrEQISstrLEQ(m,m); }
+
+       min :| min in s;
+   var done := {min};
+   var rest := s - done;
+   assert forall x <- done :: strLEQ(min, x);
+
+   while (rest > {})
+     decreases rest
+     invariant rest == (s - done)
+     invariant forall x <- done :: strLEQ(min, x)
+     invariant min in s
+     {
+      var next :| next in rest;
+      assert forall x <- done :: strLEQ(min, x);
+      if not(strLEQ(min, next)) {
+          StrNEQLEQ(min, next);
+          assert strLEQ(next, min);
+          forall x <- done ensures strLEQ( next, x)
+            { StrLEQIsTrans(next, min, x); }
+          min := next;
+          assert strLEQ(min, next);
+          assert forall x <- done :: strLEQ(min, x);
+          assert forall x <- done+{next} :: strLEQ(min, x);
+      }
+      done := done + {next};
+      rest := rest - {next};
+      assert rest == s - done;
+     }
+     assert forall x <- done :: strLEQ(min, x);
+     assert rest == {};
+     assert rest == s - done;
+     SetMinus0(s,done);
+     assert s <= done;
+     assert forall x <- s :: strLEQ(min, x);
+}
+
+
+
+
+
+
+
+lemma TEST()
+  ensures strLEQ("","")
+  ensures strLEQ("3","3")
+  ensures strLEQ("12345","12345")
+  ensures strLEQ("","oiwr")
+  ensures strLEQ("abc", "abcde")
+  ensures strLEQ("a", "z")
+  ensures strLEQ("ab", "z")
+  ensures not(strLEQ("abc","ab"))
+  ensures not(strLEQ("abzd", "abcd"))
+{}
+
+lemma STRLEQEQ(s : string)
+ ensures strLEQ(s,s)
+ {
+  if (|s| == 0)  {assert strLEQ("",""); return; }
+
+  assert |s| > 0;
+  assert not (s[0] < s[0]);
+  assert (s[0] == s[0]);
+assert (strLEQ(s[1..], s[1..]));
+
+ }
+
+predicate strLEQ(l : string, r : string)
+{
+  || (|l| == 0)
+  || (&& (|r| > 0)
+      && (|| (l[0] < r[0])
+          || ((l[0] == r[0]) && (strLEQ(l[1..], r[1..])))))
+}
+
+
+lemma StrEQISstrLEQ(l : string, r : string)
+  requires l == r
+  ensures  strLEQ(l,r)
+  {}
+
+lemma StrNEQLEQ(l : string, r : string)
+  ensures  strLEQ(l,r) || strLEQ(r,l)
+  {}
+
+lemma StrLEQLEQIsEQ(l : string, r : string)
+  requires strLEQ(l,r)
+  requires strLEQ(r,l)
+  //requires (|l| == |r| <= 1)
+  ensures  l == r
+  ensures  r == l
+  {
+    if (|l| == |r| == 0) { assert l == r; return; }
+    if (|l| == 0) { assert |r| > 0; assert not(strLEQ(r,l)); assert false; return; }
+    if (|r| == 0) { assert |l| > 0; assert not(strLEQ(l,r)); assert false; return; }
+    assert (|l| > 0) && (|r| > 0);
+    if (|l| == |r| == 1) {
+       if (l == r) { assert l == r; return; }
+       assert {:contradiction} l != r;
+       assert {:contradiction} strLEQ(l,r) != strLEQ(r,l);
+       assert {:contradiction} false;
+    }
+
+//kjx not sure why I don't need a recursie case, but it seems I don't?
+  }
+
+lemma StrLEQIsTrans(a : string, b : string, c : string)
+  requires strLEQ(a,b)
+  requires strLEQ(b,c)
+  ensures  strLEQ(a,c)
+  {}
+
+
+function fmtseqstr(Y: seq<string>) : string  //isnt this just a flatten?
+ {
+  //var Y := X;
+  if (Y == []) then ("") else (
+       Y[0] + " " + fmtseqstr( Y[1..] ) )
+  }
+//
+// lemma MSSFX(s : set<string>)
+//  requires |s| > 0
+//  ensures  exists m <- s :: forall x <- s :: strLEQ(m, x)
+//  {
+//   //  var v :| IAMTheRessurection(s, v);
+//   //  MSSFF(s, v);
+//   //  assert exists mm <- s :: ((forall x <- s :: strLEQ(mm, x)) ==> (v == mm));
+//
+//   assert |s| > 0;
+//   assert exists m :: m in s;
+//   assert exists m <- s, x <- s :: m == x;
+//
+//   forall m <- s, x <- s ensures ((m == x) ==> (strLEQ(m,x)))
+//     {
+//       if (m == x)
+//         {
+//           assert (strLEQ(m,x)) == (strLEQ(x,x)) == (strLEQ(m,m)) == (strLEQ(x,m)) == true
+//             by {
+//               STRLEQEQ(m);
+//             }
+//           assert ((m == x) ==> (strLEQ(m,x)));
+//         }
+//         else
+//         {
+//           assert m != x;
+//           assert ((m == x) ==> (strLEQ(m,x)));
+//         }
+//       assert ((m == x) ==> (strLEQ(m,x)));
+//     }
+//
+//
+//   assert exists m <- s :: exists x <- s ::   strLEQ(m,x);
+//   assert forall x <- s :: exists m <- s ::   strLEQ(m,x);
+//
+// //  assert  exists m <- s :: IAMTheRessurection(s,m); //:: forall x <- s :: strLEQ(m, x);
+//
+//  assert  exists m <- s :: forall x <- s :: strLEQ(m, x);
+//  }
+
+
+lemma MSSFF(s : set<string>, m : string)
+ requires |s| > 0
+ requires IAMTheRessurection(s, m)
+ ensures  forall x <- s :: strLEQ(m, x)
+ ensures  exists mm <- s :: ((forall x <- s :: strLEQ(mm, x)) ==> (m == mm))
+ ensures  exists m <- s :: forall x <- s :: strLEQ(m, x)
+ {}
+
+// function mss(s : set<string>) : (m : string)
+//  requires |s| > 0
+//  ensures  IAMTheRessurection(s,m)
+// {
+//   var x :| x in s && IAMTheRessurection(s,x);
+//   x
+// }
+// by method {
+//  m := minsetstr(s);
+// }
+
+
+
+lemma StringLEQ(itself : string)
+ ensures strLEQ(itself,itself)
+{}
+
+
+method minsetstr(s : set<string>) returns (m : string)
+  requires |s| > 0
+  ensures  IAMTheRessurection(s,m)
+{
+  var t := s;
+  m :| m in s;
+  var z := {m};
+  assert strLEQ(m,m) by { STRLEQEQ(m); }
+  assert m in z;
+  assert forall x <- z :: strLEQ(m,x);
+  assert IAMTheRessurection(z,m);
+
+  t := t - {m};
+
+  while t != {}
+    decreases t
+    invariant IAMTheRessurection(z,m)
+    invariant s == t + z
+  {
+    var y: string;
+    y :| y in t;
+
+assert IAMTheRessurection(z,m);
+assert (m in z && forall x | x in z && strLEQ(x, m) :: strLEQ(m, x));
+
+
+    if (strLEQ(y, m)) {
+      assert IAMTheRessurection(z,m);
+      // assert (forall x | x in (z) :: strLEQ(m, x));
+      forall x <- (z) ensures ( strLEQ(m, x) )   {  }
+      assert strLEQ(y, m);
+      forall x <- (z) ensures ( strLEQ(y, x) )   { StrLEQ2(y,m,x); }
+
+      // assert (forall x | x in (z) :: strLEQ(y, x));
+      // assert (forall x | x in (z+{y}) :: strLEQ(y, x));
+      //assert (m in (z) && forall x | x in (z+{y}) && strLEQ(x, y) ::  strLEQ(y, x));
+      assert strLEQ(y,y) by { STRLEQEQ(y); }
+      assert (y in (z+{y}) && forall x <- (z+{y}) :: strLEQ(y, x));
+      m := y;
+      assert IAMTheRessurection(z+{y},m);
+     }
+    else
+    {
+      assert not(strLEQ(y, m));
+      assert strLEQ(m, y) by { StrLEQ3(y,m); }
+      assert IAMTheRessurection(z,m);
+      assert (m in (z+{y})  && forall x <- (z+{y}) :: strLEQ(m, x));
+      assert IAMTheRessurection((z+{y}),m);
+    }
+
+
+    t := t - {y};
+    z := z + {y};
+
+    assert IAMTheRessurection(z,m);
+  }
+
+  assert IAMTheRessurection(t + z, m);
+  assert IAMTheRessurection(s, m);
+}
+
+
+
+
+
+  /** Any totally-ordered set contains a unique minimal (equivalently, least) element. */
+  lemma LemmaFindUniqueMinimal(s: set<string>) returns (min: string)
+    requires |s| > 0 // TotalOrdering(R)
+    ensures IAMTheRessurection(s, min) // && (forall min' <- s | IAMTheRessurection(s, min') :: min == min')
+  {
+    var x :| x in s;
+    if s == {x} {
+      min := x;
+      StrLEQ4(x);
+      StrLEQ4(min);
+    assert IAMTheRessurection({x}, min);
+    assert IAMTheRessurection(s, min);
+    // StrLEQ1(min, x);
+    // StrLEQ3(min, x);
+    // StrLEQ4(min);
+    // StrLEQ4(x);
+    } else {
+      var min' := LemmaFindUniqueMinimal(s - {x});
+      assert IAMTheRessurection(s - {x}, min');
+      assert forall q <- (s - {x}) :: strLEQ(min', q);
+      assert min' in (s - {x});
+      StrLEQ3(min', x);
+      if
+      case strLEQ(min', x) =>
+          assert forall q <- (s - {x}) :: strLEQ(min', q);
+          assert strLEQ(min', x);
+          assert forall q <- (s - {x} + {x}) :: strLEQ(min', q);
+          assert (s - {x}) + {x} == s;
+          assert forall q <- (s) :: strLEQ(min', q);
+          min := min';
+          assert forall q <- (s) :: strLEQ(min', q);
+          assert min in s;
+          assert forall q <- s :: strLEQ(min, q);
+          assert IAMTheRessurection(s, min);
+
+      case strLEQ(x, min') => min := x;
+          assert forall q <- (s - {x}) :: strLEQ(min', q);
+          forall q <- (s - {x}) ensures strLEQ(min, q)
+            {
+              assert strLEQ(min', q);
+              assert strLEQ(min, min');
+              StrLEQ2(min, min',q);
+            }
+          StrLEQ4(x);
+          assert min == x;
+          assert strLEQ(min, x);
+          StrLEQ4(min);
+          assert (s - {x}) + {x} == s;
+          assert IAMTheRessurection(s, min);
+    }
+    assert IAMTheRessurection(s, min);
+  }
+
+
+
+
+
+
+
+
+
+
+
+
+// method printIsomorphicOWNED(a : Object, o : Object, m : vmap<Object,Object>, os : set<Object>)
+//   decreases os
+
+//   {
+//    print "(a in m) ", (a in m), "\n";
+//    if (a !in m) { return; }
+//    var b := m[a];
+//    print "a == b ", a == b, "\n";
+//    if (a == b) { return; }
+//    print "({a,b} <= os) ",({a,b} <= os),"\n";
+//    //print "(m[a] == b) ", (m[a] == b), "\n";
+
+//    print "(recurse on owner) ", isIsomorphicMappingOWNED(a.owner, o, m, os - {a,b}),"\n";
+
+//   print "Owners overall ",
+//     isIsomorphicMappingOWNED(a.owner, o, m, os - {a,b}) ,"\n";
+
+//   print "Field names ", (a.fields.Keys == b.fields.Keys), "\n";
+
+//   if (a.fields.Keys != b.fields.Keys) {
+//       print "oops! a: ", a.fields.Keys,"\n";
+//       print "oops! b: ", b.fields.Keys,"\n";
+//       return; }
+
+//   var ns : seq<string> := set2seq(a.fields.Keys);
+
+//   for i := 0 to |ns|
+//    {
+//     var n : string := ns[i];
+//     print "  ";
+//     print "a.",n," :=";
+//     printobj(a.fields[n]);
+//     print " - ";
+//     print "b.",n," :=";
+//     printobj(b.fields[n]);
+//     print "\n";
+
+//     print "   a.",n," in m ", a.fields[n] in m, "\n";
+//     if (a.fields[n] !in m) {return;}
+//     print "   ",n," in b.fields ", n in b.fields, "\n";
+//     if (n !in b.fields) {return;}
+//     print "   b.fields[",n,"] == m[a.fields[",n,"]] ",(b.fields[n] == m[a.fields[n]]) , "\n";
+// //    print " (recurse on field ",n,") ", isIsomorphicMappingOWNED(a.fields[n], o, m, os - {a,b}),"\n";
+//    }
+// }
